now Functor and SFunctor don't use typeclasses

src/Functor.v
@@ -12,60 +12,56 @@ Ltac simplify := repeat (autounfold in *; unfold id in *; simpl in *).
 
 (* Categories *)
 
-Class FunctorData (F : Type -> Type) : Type
+Structure FunctorData (F : Type -> Type) : Type
   := { map: forall T1 T2 (f: forall (x1:T1), T2) (fx1:F T1), F T2; }.
 
-Class FunctorProp F `{FunctorData F} : Prop
+Structure FunctorProp F (Fn : FunctorData F) : Prop
   := {
       MAP_ID T:
-        map (@id T) = id;
+        Fn.(map) (@id T) = id;
       MAP_COMPOSE T1 T2 T3
                   (f12: forall (x1:T1), T2)
                   (f23: forall (x2:T2), T3)
                   x1:
-        map f23 (map f12 x1) = map (f23 ∘ f12) x1;
+        Fn.(map) f23 (Fn.(map) f12 x1) = Fn.(map) (f23 ∘ f12) x1;
     }.
-Arguments FunctorProp F {H}.
 
-Class SFunctorData F : Type
+Structure SFunctorData (F : Type -> Type) : Type
   := {
-      Functor :> FunctorData F;
+      Fn :> FunctorData F;
       mem: forall X, F X -> X -> Prop;
       map_dep: forall X Y (fx:F X) (f: forall x (MEM:mem fx x), Y), F Y;
       rel: forall X Y (rel: X -> Y -> Prop) (fx:F X) (fy:F Y), Prop;
-      MAP_DEP: forall X Y fx (f: forall x (MEM:mem fx x), Y) (g: Y -> X) (INV: forall x r, g (f x r) = x), map g (map_dep f) = fx;
+      MAP_DEP: forall X Y fx (f: forall x (MEM:mem fx x), Y) (g: Y -> X) (INV: forall x r, g (f x r) = x), Fn.(map) g (map_dep f) = fx;
     }.
-Hint Resolve MAP_DEP.
 
-Class SFunctorProp F `{SFunctorData F}
+Structure SFunctorProp F (Fn : SFunctorData F)
   : Prop
   := {
-      MAP_MEM: forall X Y (f: X -> Y) (fx: F X) (x: X) (MEM: mem fx x), mem (map f fx) (f x);
+      MAP_MEM: forall X Y (f: X -> Y) (fx: F X) (x: X) (MEM: Fn.(mem) fx x), Fn.(mem) (Fn.(map) f fx) (f x);
     }.
-Arguments SFunctorProp F {H}.
 
-Structure NatTrans (F G : Type -> Type) `{FunctorData F} `{FunctorData G} : Type :=
+Structure NatTrans (F G : Type -> Type) (FnF : FunctorData F) `(FnG : FunctorData G) : Type :=
   {
     NT :> forall {X:Type} (fx:F X), G X;
-    MAP_COMMUTE: forall T1 T2 (f:T1 -> T2) x, NT (map f x) = (map f) (NT x);
+    MAP_COMMUTE: forall T1 T2 (f:T1 -> T2) x, NT (FnF.(map) f x) = (FnG.(map) f) (NT x);
   }.
-Arguments NatTrans F G {H} {H0}.
 
-Class SNatTransProp F G `{SFunctorData F} `{SFunctorData G} `{H1 : @NatTrans F G _ _}
+Structure SNatTransProp F G (FnF : SFunctorData F) (FnG : SFunctorData G) (N : NatTrans FnF FnG)
   : Prop := {
-             MEM_COMMUTE: forall X fx (x:X), mem fx x <-> mem (H1 _ fx) x;
+             MEM_COMMUTE: forall X fx (x:X), FnF.(mem) fx x <-> FnG.(mem) (N _ fx) x;
              REL_COMMUTE: forall T1 T2 (rel': forall (x1:T1) (x2:T2), Prop) fx1 fx2,
-                 rel rel' fx1 fx2 <-> rel rel' (H1 _ fx1) (H1 _ fx2);
+                 FnF.(rel) rel' fx1 fx2 <-> FnG.(rel) rel' (N _ fx1) (N _ fx2);
            }.
 
 (* instances *)
 
 Definition Ident (X : Type) := X.
 
-Instance id_functorData : FunctorData Ident := Build_FunctorData _ (fun _ _ => id).
+Definition id_functorData : FunctorData Ident := Build_FunctorData _ (fun _ _ => id).
 
-Program Instance id_sFunctorData : SFunctorData Ident
-  := Build_SFunctorData _
+Program Definition id_sFunctorData : SFunctorData Ident
+  := Build_SFunctorData id_functorData
                         (fun _ fx x => fx = x)
                         (fun _ _ fx FX => FX _ eq_refl)
                         (fun _ _ rel fx fy => rel fx fy) _.
@@ -74,11 +70,11 @@ Hint Resolve id_functorData id_sFunctorData.
 
 Definition Const (T : Type) (X : Type) := T.
 
-Instance const_functorData T : FunctorData (Const T)
+Definition const_functorData T : FunctorData (Const T)
   := Build_FunctorData (fun X => T) (fun _ _ _ x => x).
 
-Program Instance const_sFunctorData T : SFunctorData (Const T)
-  := Build_SFunctorData _
+Program Definition const_sFunctorData T : SFunctorData (Const T)
+  := Build_SFunctorData (const_functorData T)
                         (fun _ _ _ => False)
                         (fun _ _ fx _ => fx)
                         (fun _ _ _ => eq) _.
@@ -88,33 +84,33 @@ Hint Resolve const_functorData const_sFunctorData.
 
 Definition Expn (D : Type) (F : Type -> Type) := (fun X => D -> F X).
 
-Definition function_map D F `{FunctorData F} T1 T2 (f: T1 -> T2)
+Definition function_map D F (Fn : FunctorData F) T1 T2 (f: T1 -> T2)
            (fx1: D -> F T1) :=
-  (map f) ∘ fx1.
+  (Fn.(map) f) ∘ fx1.
 Hint Unfold function_map.
 
-Inductive function_mem D F `{SFunctorData F} T (fx: D -> F T) x: Prop :=
-| Function_mem d (MEM: mem (fx d) x).
+Inductive function_mem D F (Fn : SFunctorData F) T (fx: D -> F T) x: Prop :=
+| Function_mem d (MEM: Fn.(mem) (fx d) x).
 Hint Constructors function_mem.
 
-Program Definition function_map_dep D F `{SFunctorData F} T1 T2 (fx1: D -> F T1)
-        (f: forall (x1:T1) (MEM: function_mem fx1 x1), T2): D -> F T2 :=
-  fun X => map_dep (fx1 X) (fun x MEM => (f x _)).
+Program Definition function_map_dep D F (Fn : SFunctorData F) T1 T2 (fx1: D -> F T1)
+        (f: forall (x1:T1) (MEM: function_mem Fn fx1 x1), T2): D -> F T2 :=
+  fun X => Fn.(map_dep) (fx1 X) (fun x MEM => (f x _)).
 Next Obligation.
   econstructor. eauto.
 Defined.
 
-Definition function_rel D F `{SFunctorData F} T1 T2
+Definition function_rel D F (Fn : SFunctorData F) T1 T2
            f (fx1:D -> F T1) (fx2:D -> F T2): Prop :=
-  forall d, rel f (fx1 d) (fx2 d).
+  forall d, Fn.(rel) f (fx1 d) (fx2 d).
 Hint Unfold function_rel.
 
-Instance function_functorData D F `{FunctorData F}
-  : FunctorData (Expn D F) := Build_FunctorData _ (@function_map D F _).
+Definition function_functorData D F (Fn : FunctorData F)
+  : FunctorData (Expn D F) := Build_FunctorData _ (function_map Fn).
 
-Program Instance function_sFunctorData D F `{SFunctorData F}
+Program Definition function_sFunctorData D F (Fn : SFunctorData F)
   : SFunctorData (Expn D F)
-  := Build_SFunctorData _
+  := Build_SFunctorData (function_functorData D Fn)
                         (@function_mem _ _ _)
                         (@function_map_dep _ _ _)
                         (@function_rel _ _ _) _.
@@ -127,48 +123,48 @@ Hint Resolve function_functorData function_sFunctorData.
 
 Definition Coprod (F1 F2: Type -> Type) T := (F1 T + F2 T)%type.
 
-Definition coproduct_map F1 F2 `{FunctorData F1} `{FunctorData F2} T1 T2
+Definition coproduct_map F1 F2 (Fn1 : FunctorData F1) (Fn2 : FunctorData F2) T1 T2
            (f:T1 -> T2) (fx: F1 T1 + F2 T1) :=
   match fx with
-  | inl fx => inl (map f fx)
-  | inr fx => inr (map f fx)
+  | inl fx => inl (Fn1.(map) f fx)
+  | inr fx => inr (Fn2.(map) f fx)
   end.
 
 Hint Unfold coproduct_map.
 
-Definition coproduct_mem F1 F2 `{SFunctorData F1} `{SFunctorData F2} T
+Definition coproduct_mem F1 F2 (Fn1 : SFunctorData F1) (Fn2 : SFunctorData F2) T
            (fx: F1 T + F2 T) x :=
   match fx with
-  | inl fx => mem fx x
-  | inr fx => mem fx x
+  | inl fx => Fn1.(mem) fx x
+  | inr fx => Fn2.(mem) fx x
   end.
 
 Hint Unfold coproduct_mem.
 
-Inductive coproduct_rel F1 F2 `{SFunctorData F1} `{SFunctorData F2} T1 T2 f:
+Inductive coproduct_rel F1 F2 (Fn1 : SFunctorData F1) (Fn2 : SFunctorData F2) T1 T2 r:
   forall (fx1:Coprod F1 F2 T1) (fx2:Coprod F1 F2 T2), Prop :=
-| coproduct_rel_inl fx1 fx2 (REL: rel f fx1 fx2):
-    coproduct_rel f (inl fx1) (inl fx2)
-| coproduct_rel_inr fx1 fx2 (REL: rel f fx1 fx2):
-    coproduct_rel f (inr fx1) (inr fx2)
+| coproduct_rel_inl fx1 fx2 (REL: Fn1.(rel) r fx1 fx2):
+    coproduct_rel Fn1 Fn2 r (inl fx1) (inl fx2)
+| coproduct_rel_inr fx1 fx2 (REL: Fn2.(rel) r fx1 fx2):
+    coproduct_rel Fn1 Fn2 r (inr fx1) (inr fx2)
 .
 
 Hint Constructors coproduct_rel.
 
-Program Instance coproduct_functorData  F1 F2 `{FunctorData F1} `{FunctorData F2}
+Program Definition coproduct_functorData  F1 F2 (Fn1 : FunctorData F1) (Fn2 : FunctorData F2)
   : FunctorData (Coprod F1 F2)
   := Build_FunctorData _ (@coproduct_map _ _ _ _).
 
-Program Instance coproduct_sFunctorData F1 F2 `{SFunctorData F1} `{SFunctorData F2}
+Program Definition coproduct_sFunctorData F1 F2 (Fn1 : SFunctorData F1) (Fn2 : SFunctorData F2)
   : SFunctorData (Coprod F1 F2)
-  := Build_SFunctorData _
+  := Build_SFunctorData (coproduct_functorData Fn1 Fn2)
                         (@coproduct_mem _ _ _ _)
                         _
                         (@coproduct_rel _ _ _ _) _.
 Next Obligation.
   destruct fx. 
-  - apply (inl (map_dep f0 f)).
-  - apply (inr (map_dep f0 f)).
+  - apply (inl (Fn1.(map_dep) f0 f)).
+  - apply (inr (Fn2.(map_dep) f0 f)).
 Defined.
 Next Obligation.
   destruct fx; simplify; f_equal; apply MAP_DEP; auto. 
