src/SPFunctor.v
@@ -15,9 +15,12 @@ Section UniversalFunctor.
   Variable (Sh1 Sh2: Type).
 
   Definition UF := Expn Sh1 (Coprod Ident (Const Sh2)).
-  Hint Unfold UF.
 
-  Global Instance UF_FunctorProp : FunctorProp UF.
+  Definition UF_sFunctor : SFunctorData UF :=
+    function_sFunctorData Sh1 (coproduct_sFunctorData id_sFunctorData
+                                                      (const_sFunctorData Sh2)).
+
+  Definition UF_FunctorProp : FunctorProp UF_sFunctor.
   Proof.
     constructor.
     - intro. extensionality s. extensionality s1. simplify.
@@ -27,7 +30,7 @@ Section UniversalFunctor.
   Qed.
   Hint Resolve UF_FunctorProp.
 
-  Global Instance UF_SFunctorProp : SFunctorProp UF.
+  Program Definition UF_SFunctorProp : SFunctorProp UF_sFunctor.
   Proof.
     constructor.
     intros. inv MEM. apply Function_mem with (d := d). simplify.
@@ -36,7 +39,7 @@ Section UniversalFunctor.
 
   Lemma UF_map_injective X Y (f: X -> Y) (u1 u2: UF X) 
         (INJ: forall x1 x2 (EQ: f x1 = f x2), x1 = x2)
-        (EQ: map f u1 = map f u2):
+        (EQ: UF_sFunctor.(map) f u1 = UF_sFunctor.(map) f u2):
     u1 = u2.
   Proof.
     extensionality s. apply equal_f with (x:=s) in EQ. simplify. 
@@ -45,8 +48,8 @@ Section UniversalFunctor.
   Qed.
 
   Lemma UF_map_pointwise X Y (u: UF X) (f g: X -> Y)
-        (ALL: forall x, mem u x -> f x = g x):
-    map f u = map g u.
+        (ALL: forall x, UF_sFunctor.(mem) u x -> f x = g x):
+    UF_sFunctor.(map) f u = UF_sFunctor.(map) g u.
   Proof.
     extensionality s. simplify.
     destruct (u s) eqn : EQ; auto. simplify.
@@ -55,15 +58,15 @@ Section UniversalFunctor.
   Qed.
 
   Lemma UF_rel_monotone X (u1 u2: UF X) (r r': X -> X -> Prop)
-        (LE: forall x0 x1: X, r x0 x1 -> r' x0 x1) (R: rel r u1 u2)
-        : rel r' u1 u2.
+        (LE: forall x0 x1: X, r x0 x1 -> r' x0 x1) (R: UF_sFunctor.(rel) r u1 u2)
+        : UF_sFunctor.(rel) r' u1 u2.
   Proof.
     simplify. intro d. specialize (R d).
     inv R; constructor; simplify; auto.
   Qed.
 
-  Lemma UF_map_mem X Y (f: X -> Y) (u: UF X) (x: X) (MEM: mem u x)
-        : mem (map f u) (f x).
+  Lemma UF_map_mem X Y (f: X -> Y) (u: UF X) (x: X) (MEM: UF_sFunctor.(mem) u x)
+        : UF_sFunctor.(mem) (UF_sFunctor.(map) f u) (f x).
   Proof.
     inv MEM. econstructor. instantiate (1:=d). simplify.
     destruct (u d); inversion MEM0. constructor.
@@ -73,61 +76,69 @@ End UniversalFunctor.
 
 Class SPFunctor (F : Type -> Type)
   := {
-      SFunctor :> SFunctorData F;
+      Fn :> SFunctorData F;
       Sh1 : Type;
       Sh2 : Type;
-      emb :> @NatTrans F (UF Sh1 Sh2) _ _;
-      emb_s_prop :> @SNatTransProp F (UF Sh1 Sh2) _ _ emb;
+      emb : NatTrans Fn (UF_sFunctor Sh1 Sh2);
+      emb_s_prop : SNatTransProp _ _ emb;
       INJECTIVE : forall T (x1 x2 : F T) (EQ : emb _ x1 = emb _ x2), x1 = x2;
     }.
+
+Section ddd.
+  Variable F : Type -> Type.
+
+  Coercion toSFunctor (x: SPFunctor F) : SFunctorData F := @Fn _ x.
+End ddd.
+
+Print Coercions.
 
 Section SPFunctorFacts.
 
   Variable F : Type -> Type.
-  Context `{SPFunctor F}.
+  Context `{Fn : SPFunctor F}.
 
-  Global Instance toFunctorProp : FunctorProp F.
+  Definition toFunctorProp : FunctorProp Fn.
   Proof.
     constructor.
     - intros. extensionality s.
       apply INJECTIVE.
-      rewrite MAP_COMMUTE. rewrite MAP_ID. auto.
+      rewrite MAP_COMMUTE. rewrite (UF_FunctorProp _ _).(MAP_ID). auto.
     - intros. apply INJECTIVE.
-      repeat rewrite MAP_COMMUTE. rewrite MAP_COMPOSE. auto.
+      repeat rewrite MAP_COMMUTE. rewrite (UF_FunctorProp _ _).(MAP_COMPOSE). auto.
   Qed.
 
-  Global Instance toSFunctorProp : SFunctorProp F.
+  Definition toSFunctorProp : SFunctorProp Fn.
   Proof.
     constructor. intros.
     apply (@MEM_COMMUTE _ _ _ _ _ (@emb_s_prop _ _)).
     apply (@MEM_COMMUTE _ _ _ _ _ (@emb_s_prop _ _)) in MEM.
-    rewrite (@MAP_COMMUTE _ _ _ _ (@emb _ H)).
-    apply (MAP_MEM f _ _ MEM).
+    rewrite (@MAP_COMMUTE _ _ _ _ (@emb _ Fn)).
+    apply (UF_SFunctorProp _ _).(MAP_MEM). auto.
   Qed.
 
   Lemma map_injective X Y (f: X -> Y) (u1 u2: F X)
         (INJ: forall x1 x2 (EQ: f x1 = f x2), x1 = x2)
-        (EQ: map f u1 = map f u2):
+        (EQ: Fn.(map) f u1 = Fn.(map) f u2):
     u1 = u2.
   Proof.
     apply INJECTIVE. apply (UF_map_injective INJ).
-    repeat rewrite <- MAP_COMMUTE.
-    rewrite EQ. auto.
+    repeat rewrite <- MAP_COMMUTE. simplify.
+    setoid_rewrite EQ. auto.
   Qed.
 
   Lemma map_pointwise X Y (f g: X -> Y) (m: F X)
-        (ALL: forall x, mem m x -> f x = g x):
-    map f m = map g m.
+        (ALL: forall x, Fn.(mem) m x -> f x = g x):
+    Fn.(map) f m = Fn.(map) g m.
   Proof.
     apply INJECTIVE.  repeat rewrite MAP_COMMUTE.
     apply UF_map_pointwise.
     intros. apply ALL. 
-    apply (@MEM_COMMUTE _ _ _ _ _ (@emb_s_prop _ _)). apply H0.
+    apply (@MEM_COMMUTE _ _ _ _ _ (@emb_s_prop _ _)). assumption.
   Qed.
   
   Lemma rel_monotone X (u1 u2: F X) (r r': X -> X -> Prop)
-        (LE: forall x0 x1: X, r x0 x1 -> r' x0 x1) (R: rel r u1 u2)
-    : rel r' u1 u2.
+        (LE: forall x0 x1: X, r x0 x1 -> r' x0 x1) (R: Fn.(rel) r u1 u2)
+    : Fn.(rel) r' u1 u2.
   Proof.
     apply (@REL_COMMUTE _ _ _ _ _ (@emb_s_prop _ _)).
     apply (@REL_COMMUTE _ _ _ _ _ (@emb_s_prop _ _)) in R.
