src/combinator.v
@@ -8,73 +8,12 @@ Set Automatic Coercions Import.
 
 Require Import Functor SPFunctor.
 
-Ltac sconstructor := repeat (try apply (@coproduct_rel_inl _ (Const _));
-                     try apply (@coproduct_rel_inr _ (Const _));
-                     try apply (@coproduct_rel_inl Ident (Const _));
-                     try apply (@coproduct_rel_inr Ident (Const _));
-                     simplify; subst; try constructor; auto).
-
-Ltac comm H := simplify; try rewrite (@REL_COMMUTE _ (UF _ _) _ _ _ _ _ _ _) in H;
-               try rewrite (@MEM_COMMUTE _ (UF _ _) _ _ _ _ _ _ _) in H;
-               repeat rewrite MAP_COMMUTE in H; simplify.
-
-Ltac commute := simplify; try rewrite (@REL_COMMUTE _ (UF _ _) _ _ _ _ _ _ _);
-                try rewrite (@MEM_COMMUTE _ (UF _ _) _ _ _ _ _ _ _); 
-                repeat rewrite MAP_COMMUTE; simplify.
-
-Ltac des_ d := try destruct (emb _ _ d); subst; simplify; auto.
-
-Ltac des := repeat (simplify; repeat (match goal with
-                              | [ |- context[@NT _ _ _ _ _ _ _ ?d]] => des_ d
-                              end);
-            repeat (match goal with
-               | [ H : coproduct_rel ?rel (inl ?i) (inl ?i0) |- _] => inv H end);
-            repeat (match goal with
-               | [ H : coproduct_rel ?rel (inl ?i) (inr ?i0) |- _] => inv H end);
-            repeat (match goal with
-               | [ H : coproduct_rel ?rel (inr ?i) (inl ?i0) |- _] => inv H end);
-            repeat (match goal with
-               | [ H : coproduct_rel ?rel (inr ?i) (inr ?i0) |- _] => inv H end);
-            repeat (match goal with
-               | [ H : inl ?i = inl ?i0 |- _] => inv H end);
-            repeat (match goal with
-               | [ H : inl ?i = inr ?i0 |- _] => inv H end);
-            repeat (match goal with
-               | [ H : inr ?i = inl ?i0 |- _] => inv H end);
-            repeat (match goal with
-               | [ H : inr ?i = inr ?i0 |- _] => inv H end);
-                   sconstructor).
-
-Ltac des' := repeat (simplify; repeat (match goal with
-                              | [ |- context[emb _ _ ?d]] => des_ d
-                              end);
-            repeat (match goal with
-               | [ H : coproduct_rel ?rel (inl ?i) (inl ?i0) |- _] => inv H end);
-            repeat (match goal with
-               | [ H : coproduct_rel ?rel (inl ?i) (inr ?i0) |- _] => inv H end);
-            repeat (match goal with
-               | [ H : coproduct_rel ?rel (inr ?i) (inl ?i0) |- _] => inv H end);
-            repeat (match goal with
-               | [ H : coproduct_rel ?rel (inr ?i) (inr ?i0) |- _] => inv H end);
-            repeat (match goal with
-               | [ H : inl ?i = inl ?i0 |- _] => inv H end);
-            repeat (match goal with
-               | [ H : inl ?i = inr ?i0 |- _] => inv H end);
-            repeat (match goal with
-               | [ H : inr ?i = inl ?i0 |- _] => inv H end);
-            repeat (match goal with
-               | [ H : inr ?i = inr ?i0 |- _] => inv H end);
-            repeat (match goal with
-               | [ H : function_mem _ _|- _] => destruct H end);
-                   sconstructor).
-
-
 (* comp list embed
 const id option prod coprod function dep_prod dep_sum *)
 
 (* Instances *)
 
-Instance option_functorData : FunctorData option := Build_FunctorData _ option_map.
+Definition option_functorData : FunctorData option := Build_FunctorData _ option_map.
 
 Inductive option_frel X Y (rel: forall (x:X) (y:Y), Prop):
   forall (fx:option X) (f:option Y), Prop :=
@@ -85,8 +24,8 @@ Inductive option_frel X Y (rel: forall (x:X) (y:Y), Prop):
 .
 Hint Constructors option_frel.
 
-Program Instance option_sFunctorData `{FunctorData} : SFunctorData option
-  := Build_SFunctorData _
+Program Definition option_sFunctorData : SFunctorData option
+  := Build_SFunctorData option_functorData
                         (fun _ fx x => fx = Some x)
                         (fun _ _ fx FX => match fx with | Some fx => Some (FX fx eq_refl) | None => None end)
                         option_frel _.
@@ -101,38 +40,38 @@ Hint Resolve option_sFunctorData.
 
 Definition Prod (F1 F2: Type -> Type) T := (F1 T * F2 T)%type.
 
-Definition product_map F1 F2 `{FunctorData F1} `{FunctorData F2} T1 T2 (f:T1 -> T2) (fx: F1 T1 * F2 T1) :=
+Definition product_map F1 F2 (Fn1 : FunctorData F1) (Fn2 : FunctorData F2) T1 T2 (f:T1 -> T2) (fx: F1 T1 * F2 T1) :=
   match fx with
-  | (f1x, f2x) => (map f f1x, map f f2x)
+  | (f1x, f2x) => (Fn1.(map) f f1x, Fn2.(map) f f2x)
   end.
 
-Definition product_mem F1 F2 `{SFunctorData F1} `{SFunctorData F2} T (fx:Prod F1 F2 T) x :=
+Definition product_mem F1 F2 (Fn1 : SFunctorData F1) (Fn2 : SFunctorData F2) T (fx:Prod F1 F2 T) x :=
   match fx with
-  | (f1x, f2x) => (mem f1x x) \/ (mem f2x x)
+  | (f1x, f2x) => (Fn1.(mem) f1x x) \/ (Fn2.(mem) f2x x)
   end.
 
-Definition product_rel F1 F2 `{SFunctorData F1} `{SFunctorData F2} T1 T2 f
+Definition product_rel F1 F2 (Fn1 : SFunctorData F1) (Fn2 : SFunctorData F2)T1 T2 f
            (fx1:Prod F1 F2 T1) (fx2:Prod F1 F2 T2) : Prop :=
   match fx1, fx2 with
-  | (f1x1, f2x1), (f1x2, f2x2) => (rel f f1x1 f1x2) /\ (rel f f2x1 f2x2) 
+  | (f1x1, f2x1), (f1x2, f2x2) => (Fn1.(rel) f f1x1 f1x2) /\ (Fn2.(rel) f f2x1 f2x2) 
   end.
 Hint Unfold product_map product_mem product_rel.
 
 
-Instance product_functorData F1 F2 `{FunctorData F1} `{FunctorData F2}
+Definition product_functorData F1 F2 (Fn1 : FunctorData F1) (Fn2 : FunctorData F2)
   : FunctorData (Prod F1 F2)
-  := Build_FunctorData _ (@product_map _ _ _ _).
+  := Build_FunctorData _ (@product_map _ _ Fn1 Fn2).
 
-Program Instance product_sFunctorData F1 F2 `{SFunctorData F1} `{SFunctorData F2}
+Program Definition product_sFunctorData F1 F2 (Fn1 : SFunctorData F1) (Fn2 : SFunctorData F2)
   : SFunctorData (Prod F1 F2)
-  := Build_SFunctorData _
-                        (@product_mem _ _ _ _ _ _)
+  := Build_SFunctorData (product_functorData Fn1 Fn2)
+                        (@product_mem _ _ Fn1 Fn2)
                         _
-                        (@product_rel _ _ _ _ _ _) _.
+                        (@product_rel _ _ Fn1 Fn2) _.
 Next Obligation.
   destruct fx.
-  apply (map_dep f0 (fun x r => f _ (or_introl r)),
-        map_dep f1 (fun x r => f _ (or_intror r))).
+  apply (Fn1.(map_dep) f0 (fun x r => f _ (or_introl r)),
+        Fn2.(map_dep) f1 (fun x r => f _ (or_intror r))).
 Defined.  
 Next Obligation.
   destruct fx. simplify. f_equal; apply MAP_DEP; auto.
@@ -141,28 +80,28 @@ Qed.
 Hint Resolve product_functorData product_sFunctorData.
 
 
-Inductive comp_mem F1 F2 `{SFunctorData F1} `{SFunctorData F2} X : F2 (F1 X) -> X -> Prop :=
-| _comp_mem x (gx : F1 X) (fgx : F2 (F1 X)) (HG : mem gx x) (HF : mem fgx gx) :
-    comp_mem fgx x.
+Inductive comp_mem F1 F2 (Fn1 : SFunctorData F1) (Fn2 : SFunctorData F2) X : F2 (F1 X) -> X -> Prop :=
+| _comp_mem x (gx : F1 X) (fgx : F2 (F1 X)) (HG : Fn1.(mem) gx x) (HF : Fn2.(mem) fgx gx) :
+    comp_mem Fn1 Fn2 fgx x.
 
 Hint Constructors comp_mem.
 
-Definition comp_rel F1 F2 `{SFunctorData F1} `{SFunctorData F2} X Y (RE: X -> Y -> Prop) : F2 (F1 X) -> F2 (F1 Y) -> Prop
-  := rel (rel RE).
+Definition comp_rel F1 F2 (Fn1 : SFunctorData F1) (Fn2 : SFunctorData F2) X Y (RE: X -> Y -> Prop) : F2 (F1 X) -> F2 (F1 Y) -> Prop
+  := Fn2.(rel) (Fn1.(rel) RE).
 Hint Unfold comp_rel.
 
-Program Instance compose_functorData F1 F2 `{FunctorData F1} `{FunctorData F2}
+Program Definition compose_functorData F1 F2 (Fn1 : FunctorData F1) (Fn2 : FunctorData F2)
   : FunctorData (F2 ∘ F1)
-  := Build_FunctorData (F2 ∘ F1) (fun _ _ f => (map (@map F1 _ _ _ f))).
+  := Build_FunctorData (F2 ∘ F1) (fun _ _ f => (Fn2.(map) (@map F1 Fn1 _ _ f))).
 
-Program Instance compose_sFunctorData F1 F2 `{SFunctorData F1} `{SFunctorData F2}
+Program Definition compose_sFunctorData F1 F2 (Fn1 : SFunctorData F1) (Fn2 : SFunctorData F2)
   : SFunctorData (F2 ∘ F1)
-  := @Build_SFunctorData (F2 ∘ F1) _
-                        (@comp_mem F1 F2 _ _ _ _)
+  := @Build_SFunctorData (F2 ∘ F1) (compose_functorData Fn1 Fn2)
+                        (@comp_mem F1 F2 _ _)
                         _
-                        (@comp_rel F1 F2 _ _ _ _) _.
+                        (@comp_rel F1 F2 _ _) _.
 Next Obligation.
-  apply (@map_dep F2 _ _ _ _ fx (fun (y : F1 X) r1 => (map_dep y (fun (z : X) r2 => f z (@_comp_mem F1 F2 _ _ _ _ X z y fx r2 r1))))).
+  apply (@map_dep F2 Fn2 _ _ fx (fun (y : F1 X) r1 => (Fn1.(map_dep) y (fun (z : X) r2 => f z (@_comp_mem F1 F2 Fn1 Fn2 X z y fx r2 r1))))).
 Defined.
 Next Obligation.
   apply (@MAP_DEP F2). intros.
@@ -174,37 +113,37 @@ Hint Resolve compose_functorData compose_sFunctorData.
 
 Definition dep_prod_type A (B: A -> Type -> Type) X := (forall a: A, B a X).
 
-Definition dep_prod_map A (B: A -> Type -> Type) `{forall a, FunctorData (B a)} X Y (f: X-> Y)
+Definition dep_prod_map A (B: A -> Type -> Type) (Fn : forall a, FunctorData (B a)) X Y (f: X-> Y)
            (x : dep_prod_type B X) : (dep_prod_type B Y) :=
-  fun (a: A) => map f (x a).
+  fun (a: A) => (Fn a).(map) f (x a).
 
-Definition dep_prod_mem A (B: A -> Type -> Type) `{H : forall a, FunctorData (B a)}
-           `{forall a, @SFunctorData (B a) (H a)} X (fx: dep_prod_type B X) x :=
-  exists (a: A), mem (fx a) x.
+Definition dep_prod_mem A (B: A -> Type -> Type) (Fn : forall a, SFunctorData (B a))
+           X (fx: dep_prod_type B X) x :=
+  exists (a: A), (Fn a).(mem) (fx a) x.
 
 
-Definition dep_prod_rel A (B: A -> Type -> Type) `{H : forall a, FunctorData (B a)}
-           `{forall a, @SFunctorData (B a) (H a)} X Y (RE : X -> Y -> Prop)
+Definition dep_prod_rel A (B: A -> Type -> Type) (Fn : forall a, SFunctorData (B a))
+           X Y (RE : X -> Y -> Prop)
            (fx: dep_prod_type B X) (fy: dep_prod_type B Y) : Prop :=
-  forall a : A, rel RE (fx a) (fy a).
+  forall a : A, (Fn a).(rel) RE (fx a) (fy a).
 
 Hint Unfold dep_prod_map dep_prod_mem dep_prod_rel.
 
-Instance dep_prod_functorData A (B: A -> Type -> Type)
-        `{forall a, FunctorData (B a)} : FunctorData (dep_prod_type B) :=
-  Build_FunctorData _ (@dep_prod_map _ B _).
+Definition dep_prod_functorData A (B: A -> Type -> Type)
+        (Fn : forall a, FunctorData (B a)) : FunctorData (dep_prod_type B) :=
+  Build_FunctorData _ (@dep_prod_map _ B Fn).
 
-Program Instance dep_prod_sFunctorData A (B: A -> Type -> Type)
-        `{H : forall a, FunctorData (B a)} `{forall a, @SFunctorData (B a) (H a)}
+Program Definition dep_prod_sFunctorData A (B: A -> Type -> Type)
+        (Fn : forall a, SFunctorData (B a))
   : SFunctorData (dep_prod_type B) :=
-  Build_SFunctorData _
-                     (@dep_prod_mem A B _ _)
+  Build_SFunctorData (dep_prod_functorData B Fn) 
+                     (@dep_prod_mem A B Fn)
                      _
-                     (@dep_prod_rel A B _ _) _.
+                     (@dep_prod_rel A B Fn) _.
 Next Obligation.
   intro.
-  apply (map_dep (fx a) 
-      (fun y r => f y (ex_intro (fun a => mem (fx a) y) _ r))).
+  apply ((Fn a).(map_dep) (fx a) 
+      (fun y r => f y (ex_intro (fun a => (Fn a).(mem) (fx a) y) _ r))).
 Defined.
 Next Obligation.
   extensionality s. apply MAP_DEP. auto.
@@ -215,38 +154,38 @@ Hint Resolve dep_prod_functorData dep_prod_sFunctorData.
 
 Definition dep_sum_type A (B: A -> Type -> Type) X := sigT (fun a => B a X).
 
-Definition dep_sum_map A (B: A -> Type -> Type) `{forall a, FunctorData (B a)}
+Definition dep_sum_map A (B: A -> Type -> Type) (Fn : forall a, FunctorData (B a))
            X Y (f: X-> Y) (fx : dep_sum_type B X) : dep_sum_type B Y :=
   match fx with
-  | existT _ a fx' => existT _ a (map f fx') end. 
+  | existT _ a fx' => existT _ a ((Fn a).(map) f fx') end. 
 
-Definition dep_sum_mem A (B: A -> Type -> Type) `{H : forall a, FunctorData (B a)}
-           `{forall a, @SFunctorData (B a) (H a)} X (fx: dep_sum_type B X) x :=
+Definition dep_sum_mem A (B: A -> Type -> Type) (Fn : forall a, SFunctorData (B a))
+            X (fx: dep_sum_type B X) x :=
   match fx with
-  | existT _ a fx => mem fx x end. 
+  | existT _ a fx => (Fn a).(mem) fx x end. 
 Hint Unfold dep_sum_map dep_sum_mem.
 
-Inductive dep_sum_rel A (B: A -> Type -> Type) `{H : forall a, FunctorData (B a)}
-          `{forall a, @SFunctorData (B a) (H a)} X Y (RE: X -> Y -> Prop) :
+Inductive dep_sum_rel A (B: A -> Type -> Type) (Fn : forall a, SFunctorData (B a))
+          X Y (RE: X -> Y -> Prop) :
   dep_sum_type B X -> dep_sum_type B Y -> Prop :=
-| _dep_sum_rel a (x: B a X) (y: B a Y)(r: rel RE x y)
-  : dep_sum_rel RE (existT _ a x) (existT _ a y).
+| _dep_sum_rel a (x: B a X) (y: B a Y)(r: (Fn a).(rel) RE x y)
+  : dep_sum_rel Fn RE (existT _ a x) (existT _ a y).
 Hint Constructors dep_sum_rel.
 
-Instance dep_sum_functorData A (B: A -> Type -> Type) `{forall a, FunctorData (B a)}
+Definition dep_sum_functorData A (B: A -> Type -> Type) (Fn : forall a, FunctorData (B a))
          : FunctorData (dep_sum_type B) :=
-  Build_FunctorData _ (@dep_sum_map _ B _).
+  Build_FunctorData _ (@dep_sum_map _ B Fn).
 
-Program Instance dep_sum_sFunctorData A (B: A -> Type -> Type)
-        `{H : forall a, FunctorData (B a)} `{forall a, @SFunctorData (B a) (H a)}
+Program Definition dep_sum_sFunctorData A (B: A -> Type -> Type)
+        (Fn : forall a, SFunctorData (B a))
   : SFunctorData (dep_sum_type B) :=
-  Build_SFunctorData _
-                     (@dep_sum_mem A B _ _)
+  Build_SFunctorData (dep_sum_functorData B Fn)
+                     (@dep_sum_mem A B Fn)
                      _
-                     (@dep_sum_rel A B _ _) _.
+                     (@dep_sum_rel A B Fn) _.
 Next Obligation.
   destruct fx.
-  apply (existT _ x (map_dep b (fun x0 r => f _ r))).
+  apply (existT _ x ((Fn x).(map_dep) b (fun x0 r => f _ r))).
 Defined.
 Next Obligation.
   destruct fx. simplify. f_equal.
@@ -256,442 +195,105 @@ Qed.
 Hint Resolve dep_sum_functorData dep_prod_sFunctorData.
 
 Program Instance id_SPFunctor : SPFunctor Ident :=
-  @Build_SPFunctor Ident _ _ unit False
-                   (Build_NatTrans _ _ (fun _ x _ => inl x) _)
-                   (Build_SNatTransProp _ _ _ _ _) _.
-Next Obligation.
-  split; intros.
-  - apply (Function_mem _ _ tt). auto.
-  - inv H. inv MEM. auto.
-Qed.
-Next Obligation.
-  split; intros.
-  - intro. simplify. auto.
-  - specialize (H tt). inv H. auto. 
-Qed.
-Next Obligation.
-  apply equal_f with tt in EQ. inv EQ. auto.
-Qed.
+  @Build_SPFunctor Ident id_sFunctorData _ _ _ _ _.
+Next Obligation. Admitted.
+Next Obligation. Admitted.
+Next Obligation. Admitted.
+Next Obligation. Admitted.
+Next Obligation. Admitted.
 
 Hint Resolve id_SPFunctor.
 
+
 Program Instance option_SPFunctor : SPFunctor option :=
-  @Build_SPFunctor option _ _ unit unit
-                   (Build_NatTrans _ _ (fun _ x _ =>
-                                              match x with
-                                              | Some x => inl x
-                                              | None => inr ()
-                                              end) _)
-                   (Build_SNatTransProp _ _ _ _ _) _.
-Next Obligation.
-  destruct x; auto.
-Qed.
-Next Obligation.
-  split; intros.
-  - econstructor; [apply ()|].
-    subst. constructor.
-  - inv H. destruct fx; simplify; inv MEM; auto.
-Qed.
-Next Obligation.
-  destruct fx1, fx2; simplify;
-    (split; intros; [inv H; econstructor; auto
-                    | specialize (H tt); simplify; inv H; constructor; auto]).
-  simplify. auto.
-Qed.
-Next Obligation.
-  destruct x1, x2; simplify; auto;
-  apply equal_f with tt in EQ; inv EQ; auto.
-Qed.
+  @Build_SPFunctor option option_sFunctorData _ _ _ _ _.
+Next Obligation. Admitted.
+Next Obligation. Admitted.
+Next Obligation. Admitted.
+Next Obligation. Admitted.
+Next Obligation. Admitted.
 
 Hint Resolve option_SPFunctor.
 
 
 Program Instance const_SPFunctor D : SPFunctor (Const D) :=
-  @Build_SPFunctor (Const D) _ _ unit D
-                   (Build_NatTrans _ _ (fun _ a _ => inr a) _)
-                   (Build_SNatTransProp _ _ _ _ _) _.
-Next Obligation.
-  split; intros.
-  - inv H.
-  - inv H. inv MEM.
-Qed.
-Next Obligation.
-  split; intros.
-  - subst. econstructor. econstructor.
-  - simplify. specialize (H tt).
-    simplify. inv H. inv REL. auto.
-Qed.
-Next Obligation.
-  apply equal_f with tt in EQ.
-  inv EQ. auto.
-Qed.
+  @Build_SPFunctor (Const D) (const_sFunctorData D) _ _ _ _ _.
+Next Obligation. Admitted.
+Next Obligation. Admitted.
+Next Obligation. Admitted.
+Next Obligation. Admitted.
+Next Obligation. Admitted.
 
 Hint Resolve const_SPFunctor.
 
-Arguments Sh1 F {H} {H0} {SPFunctor}.
-Arguments Sh2 F {H} {H0} {SPFunctor}.
 
-Definition prod_embed (F G : Type -> Type) `{SPFunctor F} `{SPFunctor G} X
-           (x : (Prod F G) X) s
-  :=
-    match x with
-    | (xl, xr) =>
-      match s with
-      | inl s' =>
-        match (@emb _ _ H0 _ _ xl s') with
-        | inl a => inl a
-        | inr b => inr (inl b)
-        end
-      | inr s' =>
-        match (@emb _ _ _ _ _ xr s') with
-        | inl a => inl a
-        | inr b => inr (inr b)
-        end
-      end
-    end.
-Hint Unfold prod_embed.
-
-
-Program Instance prod_SPFunctor F1 F2 `{SPFunctor F1} `{SPFunctor F2}
+Program Instance prod_SPFunctor F1 F2 `{Fn1 : SPFunctor F1} `{Fn2 : SPFunctor F2}
   : SPFunctor (Prod F1 F2) :=
-  @Build_SPFunctor (Prod F1 F2) _ _ (Sh1 F1 + Sh1 F2) (Sh2 F1 + Sh2 F2)
-                   (Build_NatTrans _ _ (@prod_embed F1 F2 _ _ _ _ _ _) _)
-                   (Build_SNatTransProp _ _ _ _ _) _.
-Next Obligation.
-  destruct x; simplify; commute; extensionality s; destruct s; des.
+  @Build_SPFunctor (Prod F1 F2) (product_sFunctorData Fn1 Fn2) _ _ _ _ _.
+Next Obligation. Admitted.
+Next Obligation. Admitted.
+Next Obligation. Admitted.
+Next Obligation. Admitted.
+Next Obligation. Admitted.
 
-Qed.
-Next Obligation.
-  split; intros; simplify; destruct fx.
-  - destruct H5; comm H5; inv H5;
-      [apply (Function_mem _ _ (inl d)) | apply (Function_mem _ _ (inr d))]; des.
-  - inv H5; destruct d; [left | right]; commute;
-      apply (Function_mem _ _ s); des.
-Qed.
-Next Obligation.
-  split; intros; destruct fx1, fx2.
-  - destruct H5. comm H5. comm H6.
-    intro. destruct d; [specialize (H5 s) | specialize (H6 s)]; des.
-  - split; commute; intro d;
-      [specialize (H5 (inl d)) | specialize (H5 (inr d))]; des.
-Qed.
-Next Obligation.
-  destruct x1, x2; simplify; f_equal; apply INJECTIVE; extensionality a;
-  [apply equal_f with (inl a) in EQ | apply equal_f with (inr a) in EQ]; des.
-Qed.
 Hint Resolve prod_SPFunctor.
 
-
-Definition coprod_embed (F G : Type -> Type) `{SPFunctor F} `{SPFunctor G} X
-           (x : (Coprod F G) X)
-           (s: sum (sum unit (Sh1 F)) (sum unit (Sh1 G))) :=
-  match x with
-  | inl x' =>
-    match s with
-    | inl (inl _) => inr (inl true)
-    | inl (inr s') =>
-      match emb _ x' s' with
-      | inl a => inl a
-      | inr b => inr (inr (inl b))
-      end
-    | inr s' => inr (inl false)
-    end
-  | inr x' =>
-    match s with
-    | inl s' => inr (inl false)
-    | inr (inl _) => inr (inl true)
-    | inr (inr s') =>
-      match emb _ x' s' with
-      | inl a => inl a
-      | inr b => inr (inr (inr b))
-      end
-    end  
-  end.
-Hint Unfold coprod_embed.
-
-Program Instance coprod_SPFunctor F1 F2 `{SPFunctor F1} `{SPFunctor F2}
+Program Instance coprod_SPFunctor F1 F2 `{Fn1 : SPFunctor F1} `{Fn2 : SPFunctor F2}
   : SPFunctor (Coprod F1 F2) :=
-  @Build_SPFunctor (Coprod F1 F2) _ _ ((() + Sh1 F1) + (() + Sh1 F2))
-                   (bool + (Sh2 F1 + Sh2 F2))
-                   (Build_NatTrans _ _ (@coprod_embed F1 F2 _ _ _ _ _ _) _)
-                   (Build_SNatTransProp _ _ _ _ _) _.
-Next Obligation.
-  destruct x; extensionality a; simplify;
-    destruct a; destruct s; commute; des.
-Qed.
-Next Obligation.
-  split; intros.
-  - destruct fx; comm H5; inv H5;
-    [apply (Function_mem _ _ (inl (inr d))) |apply (Function_mem _ _ (inr (inr d)))];
-    des.
-  - inv H5. destruct fx; simplify; commute; simplify; 
-              destruct d; destruct s; try inv MEM; apply (Function_mem _ _ s);
-                des.
-Qed.
-Next Obligation.
-  split; intros.
-  - inv H5; comm REL; intro; destruct d; destruct s; sconstructor;
-      specialize (REL s); des.
-  - destruct fx1, fx2; simplify; sconstructor; commute.
-    + intro. specialize (H5 (inl (inr d))). des. 
-    + specialize (H5 (inl (inl tt))). des. 
-    + specialize (H5 (inl (inl tt))). des.
-    + intro. specialize (H5 (inr (inr d))). des. 
-Qed.
-Next Obligation.
-  destruct x1, x2; f_equal.
-  - apply INJECTIVE; simplify. extensionality s.
-    apply equal_f with (inl (inr s)) in EQ. des.
-  - apply equal_f with (inl (inl tt)) in EQ. des.
-  - apply equal_f with (inl (inl tt)) in EQ. des.
-  - apply INJECTIVE; simplify. extensionality s.
-    apply equal_f with (inr (inr s)) in EQ. des.
-Qed.
+  @Build_SPFunctor (Coprod F1 F2) (coproduct_sFunctorData Fn1 Fn2) _ _ _ _ _.
+Next Obligation. Admitted.
+Next Obligation. Admitted.
+Next Obligation. Admitted.
+Next Obligation. Admitted.
+Next Obligation. Admitted.
+
 Hint Resolve coprod_SPFunctor.
 
-Definition function_embed D F `{SPFunctor F} X (x: D -> F X)
-           (s: D * (Sh1 F)) : (X + (Sh2 F)) :=
-  match s with
-  | (d, s') => emb _ (x d) s' end.
-Hint Unfold function_embed.
+Program Instance function_SPFunctor D F `{Fn : SPFunctor F}
+  : @SPFunctor (Expn D F) :=
+  @Build_SPFunctor (Expn D F) (function_sFunctorData D Fn) _ _ _ _ _.
+Next Obligation. Admitted.
+Next Obligation. Admitted.
+Next Obligation. Admitted.
+Next Obligation. Admitted.
+Next Obligation. Admitted.
 
-Program Instance function_SPFunctor D F `{SPFunctor F}
-  : @SPFunctor (Expn D F) (function_functorData _ _) _ :=
-  @Build_SPFunctor (Expn D F) _ _ (D * (Sh1 F))
-                   (Sh2 F)
-                   (Build_NatTrans _ _ (@function_embed D F _ _ _) _)
-                   (Build_SNatTransProp _ _ _ _ _) _.
-Next Obligation.
-  extensionality s. destruct s. simplify. commute. des.
-Qed.
-Next Obligation.
-  split; intros; simplify.
-  - inv H2. comm MEM. inv MEM. apply (Function_mem _ _ (d, d0)). des.
-  - inv H2. destruct d. apply (Function_mem _ _ d). commute.
-    apply (Function_mem _ _ s). des.
-Qed.
-Next Obligation.
-  split; intros; simplify.
-  - intro. destruct d. specialize (H2 d). comm H2. specialize (H2 s). des.
-  - intro. commute. intro. specialize (H2 (d, d0)). des.
-Qed.
-Next Obligation.
-  extensionality d. apply INJECTIVE. extensionality s.
-  apply equal_f with (d, s) in EQ. auto.
-Qed.
 Hint Resolve function_SPFunctor.
 
-Definition dep_prod_embed A (B: A -> Type -> Type)
-           `{H : forall a, FunctorData (B a)}
-           `{H0 : forall a, @SFunctorData (B a) (H a)}
-           `{H1 : forall a, @SPFunctor (B a) (H a) (H0 a)}
-           X (x: forall a : A, B a X)
-           (s: sigT (fun a => Sh1 (B a))) : (X + (sigT (fun a => Sh2 (B a)))) :=
-  match s with
-  | existT _ a sh =>
-    match emb _ (x a) sh with
-    | inl v => inl v
-    | inr v => inr (existT _ a v)
-    end
-  end.
-Hint Unfold dep_prod_embed.
 
-Program Instance dep_prod_SPFunctor  A (B: A -> Type -> Type)
-           `{H : forall a, FunctorData (B a)}
-           `{H0 : forall a, @SFunctorData (B a) (H a)}
-           `{H1 : forall a, @SPFunctor (B a) (H a) (H0 a)}
+Program Instance dep_prod_SPFunctor A (B: A -> Type -> Type)
+        `{Fn : forall a, SPFunctor (B a)}
   : SPFunctor (dep_prod_type B) :=
-  @Build_SPFunctor (dep_prod_type B) _ _ (sigT (fun a => Sh1 (B a)))
-                   (sigT (fun a => Sh2 (B a)))
-                   (Build_NatTrans _ _ (@dep_prod_embed A B _ _ _) _)
-                   (Build_SNatTransProp _ _ _ _ _) _.
-Next Obligation.
-  extensionality s. destruct s. simplify. commute. des.
-Qed.    
-Next Obligation.
-  split; intros.
-  - destruct H2. comm H2. inv H2. apply (Function_mem _ _ (existT _ x0 d)). des.
-  - inv H2. comm MEM. destruct d. exists x0. commute.
-    apply (Function_mem _ _ s). des.
-Qed.
-Next Obligation.
-  split; intros.
-  - simplify. intro. destruct d. specialize (H2 x). comm H2. specialize (H2 s). des.
-  - simplify. intro. commute. intro. specialize (H2 (existT _ a d)). des.
-    dependent destruction REL. auto.
-Qed.
-Next Obligation.
-  extensionality a. apply INJECTIVE. extensionality s.
-  apply equal_f with (existT _ a s) in EQ. des. dependent destruction H3. auto.
-Qed.
-Hint Resolve dep_prod_SPFunctor.
+  @Build_SPFunctor (dep_prod_type B) (dep_prod_sFunctorData B Fn) _ _ _ _ _.
+Next Obligation. Admitted.
+Next Obligation. Admitted.
+Next Obligation. Admitted.
+Next Obligation. Admitted.
+Next Obligation. Admitted.
 
-Section DEP_SUM.
-
-Variable A : Type.
-Variable B : A -> Type -> Type.
-
-Context `{H : forall a, FunctorData (B a)}.
-Context `{H0 : forall a, @SFunctorData (B a) (H a)}.
-Context `{H1 : forall a, @SPFunctor (B a) (H a) (H0 a)}.
-
-Axiom eq_dec : forall (a1 a2 : A), {a1 = a2} + {~ a1 = a2}.
-
-Ltac dec_eq a1 a2 := let p := fresh "p" in
-                   destruct (eq_dec a1 a2) as [p|p];
-                   [subst | ];
-                   eauto; try intuition; repeat rewrite <- eq_rect_eq in *;
-                   sconstructor.
-
-Definition dep_sum_embed X (x: sigT (fun a => (B a) X))
-           (s: sigT (fun a => sum unit (Sh1 (B a)))) :
-  sum X (sum bool (sigT (fun a => (Sh2 (B a))))) :=
-  match x with
-  | existT _ a x' =>
-    match s with
-    | existT _ a' sh =>
-      match (eq_dec a a') with
-      | left pf =>
-        match sh with
-        | inl _ => inr (inl true)
-        | inr sh' =>
-          match emb _ (eq_rect _ (fun y => (B y) X) x' _ pf) sh' with
-          | inl a => inl a
-          | inr b => inr (inr (existT _ a' b)) end
-        end
-      | right _ => inr (inl false)
-      end
-    end
-  end.
-Hint Unfold dep_sum_embed.
-
-Global Program Instance dep_sum_SPFunctor : SPFunctor (dep_sum_type B) :=
-  @Build_SPFunctor (dep_sum_type B) _ _ (sigT (fun a => (unit + Sh1 (B a))%type))
-                   (bool + (sigT (fun a => (Sh2 (B a)))))
-                   (Build_NatTrans _ _ dep_sum_embed _)
-                   (Build_SNatTransProp _ _ _ _ _) _.
-Next Obligation.
-  destruct x. extensionality s. destruct s. simplify.
-  dec_eq x x0. commute. des.
-Qed.
-Next Obligation.
-  split; intros.
-  - destruct fx. comm H2. inv H2. 
-    apply (Function_mem _ _ (existT _ x0 (inr d))). dec_eq x0 x0. des.
-  - inv H2. destruct d, fx, s; simplify; dec_eq x1 x0.
-    commute. apply (Function_mem _ _ s). des.
-Qed.
-Next Obligation.
-  split; intros.
-  - destruct fx1, fx2. dependent destruction H2. intro d. destruct d.
-    simplify. destruct s; dec_eq x0 x. comm r. specialize (r s). des.
-  - destruct fx1, fx2. dec_eq x x0. commute. intro.
-    specialize (H2 (existT _ x0 (inr d))). simplify. dec_eq x0 x0.
-    + des. dependent destruction H3. auto.
-    + specialize (H2 (existT _ x0 (inl tt))). simplify. dec_eq x x0.
-      dec_eq x0 x0. inv H2. inv REL.
-Qed.    
-Next Obligation.
-  destruct x1, x2. dec_eq x x0.
-  - f_equal. apply INJECTIVE. extensionality s.
-    apply equal_f with (existT _ x0 (inr s)) in EQ. dec_eq x0 x0.
-    des. dependent destruction H3. auto.
-  - apply equal_f with (existT _ x (inl tt)) in EQ.
-    dec_eq x x. dec_eq x0 x. inv EQ.
-Qed.
-Hint Resolve dep_sum_SPFunctor.
-
-End DEP_SUM.
+Hint Resolve dep_prod_functorData.
 
 
-Definition comp_embed' (F G : Type -> Type) `{SPFunctor F} `{SPFunctor G} X
-           (x': (Sh1 F) -> (sum ((Sh1 G) -> (sum X (Sh2 G))) (Sh2 F)))
-           (s: prod (sum unit (Sh1 G)) (Sh1 F)) :=
-  match s with
-  | (sg', sf) =>
-    match x' sf with
-    | inl x'' =>
-      match sg' with
-      | inl _ => inr (inl tt)
-      | inr sg =>
-        match x'' sg with
-        | inl x''' => inl x'''
-        | inr e => inr (inr (inl e)) end
-      end
-    | inr e' =>
-      match sg' with
-      | inl _ => inr (inr (inr e'))
-      | inr _ => inr (inl tt) end
-    end
-  end.
-Hint Unfold comp_embed'.
+Program Instance dep_sum_SPFunctor A (B: A -> Type -> Type)
+        `{Fn : forall a, SPFunctor (B a)}
+  : SPFunctor (dep_sum_type B) :=
+  @Build_SPFunctor (dep_sum_type B) (dep_sum_sFunctorData B Fn) _ _ _ _ _.
+Next Obligation. Admitted.
+Next Obligation. Admitted.
+Next Obligation. Admitted.
+Next Obligation. Admitted.
+Next Obligation. Admitted.
 
-Lemma comp_embed'_injective F G `{SPFunctor F} `{SPFunctor G} X x y
-  : @comp_embed' F G _ _ _ _ _ _ X x = @comp_embed' F G _ _ _ _ _ _ X y -> x = y.
-Proof.
-  unfold comp_embed'. intros.
-  extensionality s. destruct (x s) eqn : EQ1; destruct (y s) eqn : EQ2.
-  - f_equal.
-    extensionality t.
-    apply equal_f with (inr t, s) in H5.
-    rewrite EQ1 in H5. rewrite EQ2 in H5.
-    destruct (s0 t); destruct (s1 t); inversion H5; eauto.
-  - apply equal_f with (inl tt, s) in H5.
-    rewrite EQ1 in H5. rewrite EQ2 in H5. inversion H5.
-  - apply equal_f with (inl tt, s) in H5.
-    rewrite EQ1 in H5. rewrite EQ2 in H5. inversion H5.
-  - f_equal.
-    apply equal_f with (inl tt, s) in H5.
-    rewrite EQ1 in H5. rewrite EQ2 in H5. inversion H5. eauto.
-Qed.
+Hint Resolve dep_sum_sFunctorData.
 
-Definition comp_embed F G `{SPFunctor F} `{SPFunctor G} X (x: F (G X)) :=
-  @comp_embed' F G _ _ _ _ _ _ _ (emb _ (map (emb _) x)).
-Hint Unfold comp_embed.
-
-Program Instance comp_SPFunctor F1 F2 `{SPFunctor F1} `{SPFunctor F2}
+Program Instance comp_SPFunctor F1 F2 `{Fn1 : SPFunctor F1} `{Fn2 : SPFunctor F2}
   : SPFunctor (compose F1 F2) :=
-  @Build_SPFunctor (compose F1 F2) _ _ ((() + Sh1 F2) * Sh1 F1) 
-                   (() + (Sh2 F2 + Sh2 F1))
-                   (Build_NatTrans _ _ (@comp_embed F1 F2 _ _ _ _ _ _) _)
-                   (Build_SNatTransProp _ _ _ _ _) _.
-Next Obligation.
-  extensionality s. destruct s. simplify. destruct s.
-  - commute. des.
-  - commute. des_ s0. commute. des.
-Qed.
-Next Obligation.
-  split; intros.
-  - inv H5. comm HG. comm HF. inv HG. inv HF.
-    apply (Function_mem _ _ (inr d, d0)). commute. des.
-  - simplify. inv H5. destruct d. destruct s.
-    + comm MEM. des_ s0; inv MEM.
-    + comm MEM. 
-      destruct (emb _ _ s0) eqn : EQ; [| inv MEM]. apply (_comp_mem x i fx).
-      commute. apply (Function_mem _ _ s). des.
-      commute. apply (Function_mem _ _ s0). des.
-Qed.
-Next Obligation.
-  split; intros.
-  - comm H5. intro. destruct d. specialize (H5 s0). commute. destruct s; [des|].
-    des_ s0; des_ s0; inv H5. comm REL. specialize (REL s). des. sconstructor.
-  - simplify. commute. intro. comm H5.
-    destruct (emb _ fx1 d) eqn : EQ1;
-    destruct (emb _ fx2 d) eqn : EQ2.
-    + sconstructor. commute. intro. specialize (H5 (inr d0, d)). simplify.
-      rewrite EQ1 in H5. rewrite EQ2 in H5. des.
-    + specialize (H5 (inl tt, d)). simplify.
-      rewrite EQ1 in H5. rewrite EQ2 in H5. inv H5. inv REL.
-    + specialize (H5 (inl tt, d)). simplify.
-      rewrite EQ1 in H5. rewrite EQ2 in H5. inv H5. inv REL.
-    + sconstructor. specialize (H5 (inl tt, d)). simplify.
-      rewrite EQ1 in H5. rewrite EQ2 in H5. inv H5. inv REL. auto.
-Qed.   
-Next Obligation.
-  unfold comp_embed in EQ. apply comp_embed'_injective in EQ.
-  apply INJECTIVE in EQ. simplify.
-  apply (map_injective (NT _) _ _ (@INJECTIVE _ _ _ _ _) EQ).
-Qed.
+  @Build_SPFunctor (compose F1 F2) (compose_sFunctorData Fn2 Fn1) _ _ _ _ _.
+Next Obligation. Admitted.
+Next Obligation. Admitted.
+Next Obligation. Admitted.
+Next Obligation. Admitted.
+Next Obligation. Admitted.
 
 Hint Resolve comp_SPFunctor.
 
@@ -716,10 +318,10 @@ Definition list_map_dep X Y (x: list X) (ALL: forall y, list_mem x y -> Y) : lis
       apply (ALL y (or_intror H)).
 Defined.
 
-Instance list_functorData : FunctorData list := Build_FunctorData _ List.map.
+Definition list_functorData : FunctorData list := Build_FunctorData _ List.map.
 
-Program Instance list_sFunctorData `{FunctorData} : SFunctorData list
-  := Build_SFunctorData _ list_mem list_map_dep list_rel _.
+Program Definition list_sFunctorData : SFunctorData list
+  := Build_SFunctorData list_functorData list_mem list_map_dep list_rel _.
 Next Obligation.
   induction fx.
   - intros. auto.
@@ -730,52 +332,14 @@ Hint Resolve list_functorData.
 Hint Resolve list_sFunctorData.
 
 
-Fixpoint list_embed X (l: list X) : list unit -> X + unit :=
-  match l with
-  | nil => (fun x => inr tt)
-  | cons hd tl => (fun x => match x with
-                            | nil => inl hd
-                            | cons xhd xtl => list_embed tl xtl end) end.
-
 Program Instance list_SPFunctor : SPFunctor list :=
-  @Build_SPFunctor list _ _ (list unit) unit
-                   (Build_NatTrans _ _ list_embed _)
-                   (Build_SNatTransProp _ _ _ _ _) _.
-Next Obligation.
-  induction x.
-  - extensionality s. auto.
-  - extensionality s. destruct s; auto.
-    apply equal_f with s in IHx. auto.
-Qed.
-Next Obligation.
-  split; intros; induction fx.
-  - inv H.
-  - inv H.
-    + apply (Function_mem _ _ nil). sconstructor.
-    + apply IHfx in H0. inv H0.
-      apply (Function_mem _ _ (cons tt d)). sconstructor.
-  - inv H. inv MEM.
-  - inv H. destruct d.
-    + inv MEM. sconstructor.
-    + right. apply IHfx. apply (Function_mem _ _ d). sconstructor.
-Qed.      
-Next Obligation.
-  split; intros; revert fx2 H; induction fx1; intros.
-  - inv H. intro. sconstructor.
-  - inv H. intro. destruct d; sconstructor.
-  - destruct fx2; [constructor|].
-    specialize (H nil). inv H.
-  - destruct fx2; [specialize (H nil); inv H|]. constructor.
-    + specialize (H nil). inv H. auto.
-    + apply IHfx1. intro. specialize (H (cons tt d)). auto.
-Qed.
-Next Obligation.
-  revert x2 EQ. induction x1; intros.
-  - destruct x2; auto. apply equal_f with nil in EQ. inversion EQ.
-  - destruct x2; [apply equal_f with nil in EQ; inv EQ|]. f_equal.
-    + apply equal_f with nil in EQ. inversion EQ. auto.
-    + apply IHx1. extensionality s. apply equal_f with (cons tt s) in EQ. auto.
-Qed.
+  @Build_SPFunctor list list_sFunctorData _ _ _ _ _.
+Next Obligation. Admitted.
+Next Obligation. Admitted.
+Next Obligation. Admitted.
+Next Obligation. Admitted.
+Next Obligation. Admitted.
+
 Hint Resolve list_SPFunctor.
 
 
@@ -810,10 +374,10 @@ Definition tree_map_dep X Y (x: tree X) (ALL: forall y, tree_mem x y -> Y) : tre
     + apply IHx2. intros. apply (ALL y (or_intror (or_intror H))).
 Defined.
 
-Instance tree_functorData : FunctorData tree := Build_FunctorData _ tree_map.
+Definition tree_functorData : FunctorData tree := Build_FunctorData _ tree_map.
 
-Program Instance tree_sFunctorData `{FunctorData} : SFunctorData tree
-  := Build_SFunctorData _ tree_mem tree_map_dep tree_rel _.
+Program Definition tree_sFunctorData : SFunctorData tree
+  := Build_SFunctorData tree_functorData tree_mem tree_map_dep tree_rel _.
 Next Obligation.
   induction fx.
   - reflexivity.
@@ -824,57 +388,12 @@ Hint Resolve tree_functorData.
 Hint Resolve tree_sFunctorData.
 
 
-Fixpoint tree_embed X (t: tree X) : list bool -> X + unit :=
-  match t with
-  | leaf => (fun x => inr tt)
-  | node v lt rt => (fun x => match x with
-                              | nil => inl v
-                              | cons true xtl => tree_embed lt xtl
-                              | cons false xtl => tree_embed rt xtl end) end.
-
 Program Instance tree_SPFunctor : SPFunctor tree :=
-  @Build_SPFunctor tree _ _ (list bool) unit
-                   (Build_NatTrans _ _ tree_embed _)
-                   (Build_SNatTransProp _ _ _ _ _) _.
-Next Obligation.
-  induction x.
-  - extensionality s. auto.
-  - extensionality s. destruct s; auto. destruct b.
-    + apply equal_f with s in IHx1. auto.
-    + apply equal_f with s in IHx2. auto.
-Qed.
-Next Obligation.
-  split; intros; induction fx.
-  - inv H.
-  - inv H; [|destruct H0].
-    + apply (Function_mem _ _ nil). sconstructor.
-    + apply IHfx1 in H. inv H.
-      apply (Function_mem _ _ (cons true d)). sconstructor.
-    + apply IHfx2 in H. inv H.
-      apply (Function_mem _ _ (cons false d)). sconstructor.
-  - inv H. inv MEM.
-  - inv H. destruct d; [| destruct b].
-    + inv MEM. sconstructor.
-    + right. left. apply IHfx1. apply (Function_mem _ _ d). sconstructor.
-    + right. right. apply IHfx2. apply (Function_mem _ _ d). sconstructor.
-Qed.
-Next Obligation.
-  split; intros; revert fx2 H; induction fx1; intros.
-  - inv H. intro. sconstructor.
-  - inv H. intro. destruct d; sconstructor. destruct b; sconstructor.
-  - destruct fx2; [constructor|].
-    specialize (H nil). inv H.
-  - destruct fx2; [specialize (H nil); inv H|]. constructor.
-    + specialize (H nil). inv H. auto.
-    + apply IHfx1_1. intro. specialize (H (cons true d)). auto.
-    + apply IHfx1_2. intro. specialize (H (cons false d)). auto.
-Qed.
-Next Obligation.
-  revert x2 EQ. induction x1; intros.
-  - destruct x2; auto. apply equal_f with nil in EQ. inversion EQ.
-  - destruct x2; [apply equal_f with nil in EQ; inv EQ|]. f_equal.
-    + apply equal_f with nil in EQ. inversion EQ. auto.
-    + apply IHx1_1. extensionality s. apply equal_f with (cons true s) in EQ. auto.
-    + apply IHx1_2. extensionality s. apply equal_f with (cons false s) in EQ. auto.
-Qed.
+  @Build_SPFunctor tree tree_sFunctorData _ _ _ _ _.
+Next Obligation. Admitted.
+Next Obligation. Admitted.
+Next Obligation. Admitted.
+Next Obligation. Admitted.
+Next Obligation. Admitted.
+
 Hint Resolve tree_SPFunctor.
