src/monad.v
@@ -8,164 +8,157 @@ Set Automatic Coercions Import.
 
 Require Import Functor SPFunctor combinator spec inductive.
 
-Class Monad (F : Type -> Type) `{FunctorData F} :=
-  {  
-    ret :> NatTrans Ident F;
-    mult :> NatTrans (F ∘ F) F;
+Class Monad {F : Type -> Type} (Fn : FunctorData F) :=
+  { 
+    ret : NatTrans id_functorData Fn;
+    mult : NatTrans (compose_functorData Fn Fn) Fn;
     monad_law_1 : forall X (x : F (F (F X))), 
-        (mult X) (mult (F X) x) = (mult X) (@map _ H _ _ (mult X) x);
+        (mult X) (mult (F X) x) = (mult X) (@map _ Fn _ _ (mult X) x);
     monad_law_2 : forall X (x : F X),
-        (mult X) (map (ret X) x) = x;
+        (mult X) (Fn.(map) (ret X) x) = x;
     monad_law_3 : forall X (x : F X), (mult X) (ret (F X) x) = x;
   }.
 
-Class SMonad F `{FunctorData F} `{@SFunctorData F _} `{@SPFunctor F _ _} `{@Monad F _} := {}.
+Section monad.
 
-Definition bind M `{SMonad M} {X Y} (f: X -> M Y) (x: M X) :=
-  mult Y (map f x).
-Hint Unfold bind.
+  Variable M : Type -> Type.
+  Context `{Fn : SPFunctor M}.
+  Context `{Monad M Fn}.
 
-Lemma bind_law_1 M `{SMonad M} X Y (f: X -> M Y) x : bind f (ret X x) = f x.
-Proof.
-  intros. unfold bind. rewrite <- MAP_COMMUTE. apply monad_law_3.
-Qed.
+  Definition bind {X Y} (f: X -> M Y) (x: M X) :=
+    mult Y (Fn.(map) f x).
+  Hint Unfold bind.
 
-Lemma bind_law_2 M `{SMonad M} X x : bind (ret X) x = x.
-Proof.
-  apply monad_law_2.
-Qed.
+  Lemma bind_law_1 X Y (f: X -> M Y) x : bind f (ret X x) = f x.
+  Proof.
+    intros. unfold bind. rewrite <- MAP_COMMUTE. apply monad_law_3.
+  Qed.
 
-Lemma bind_law_3 M `{SMonad M} X Y Z (f : X -> M Y) (g : Y -> M Z) x :
+  Lemma bind_law_2 X x : bind (ret X) x = x.
+  Proof.
+    apply monad_law_2.
+  Qed.
+
+  Lemma bind_law_3 X Y Z (f : X -> M Y) (g : Y -> M Z) x :
     (bind g) ((bind f) x) = bind (fun x0 => bind g (f x0)) x.
-Proof.
-  unfold bind.
-  rewrite <- MAP_COMMUTE. rewrite monad_law_1. simplify.
-  repeat rewrite MAP_COMPOSE. auto. 
-Qed.
+  Proof.
+    unfold bind.
+    rewrite <- MAP_COMMUTE. rewrite monad_law_1. simplify.
+    repeat rewrite (@MAP_COMPOSE _ _ (@toFunctorProp _ Fn)). auto.     
+  Qed.
 
-Lemma bind_lemma_1 M `{SMonad M} X (x : M (M X)) : mult X x = bind id x.
-Proof.
-  unfold bind.
-  rewrite MAP_ID. auto.
-Qed.
+  Lemma bind_lemma_1 X (x : M (M X)) : mult X x = bind id x.
+  Proof.
+    unfold bind.
+    rewrite (@MAP_ID _ _ (@toFunctorProp _ Fn)). auto.
+  Qed.
 
-Lemma bind_lemma_2 M `{SMonad M} X Y (f: X -> Y) x :
-    map f x = bind (fun y => ret _ (f y)) x.
-Proof.
-  unfold bind. simplify.
-  setoid_rewrite <- MAP_COMPOSE.
-  setoid_rewrite monad_law_2. rewrite MAP_ID. auto.
-Qed.
+  Lemma bind_lemma_2 X Y (f: X -> Y) x :
+    Fn.(map) f x = bind (fun y => ret _ (f y)) x.
+  Proof.
+    unfold bind. simplify.
+    setoid_rewrite <- (@MAP_COMPOSE _ _ (@toFunctorProp _ Fn)).
+    setoid_rewrite monad_law_2. rewrite (@MAP_ID _ _ (@toFunctorProp _ Fn)). auto.
+  Qed.
 
+  Variable X : Type.
 
-Section Mlist.
+  Definition F := Coprod (Const unit) (Prod (Const (M X)) M).
 
-Variable M : Type -> Type.
-Context `{SMonad M}.
-Variable X : Type.
+  Definition Mlist := ffix F.
 
-Definition F := Coprod (Const unit) (Prod (Const (M X)) M).
+  Definition Mnil := Ffix F (inl tt).
+  Definition Mcons (hd : M X) (tl : M Mlist) := Ffix F (inr (hd, tl)).
 
-Definition Mlist := ffix F.
+  Lemma Mcons_inj h1 t1 h2 t2
+        (EQ: Mcons h1 t1 = Mcons h2 t2):
+    h1 = h2 /\ t1 = t2.
+  Proof.
+    unfold Mcons in *. apply Ffix_inj in EQ. inversion EQ. auto.
+  Qed.
 
-Definition Mnil := Ffix F (inl tt).
-Definition Mcons (hd : M X) (tl : M Mlist) := Ffix F (inr (hd, tl)).
+  Lemma Mcons_inj2 hd tl (EQ: Mcons hd tl = Mnil):
+    False.
+  Proof.
+    unfold Mcons, Mnil in *. apply Ffix_inj in EQ. inversion EQ.
+  Qed.
 
-Lemma Mcons_inj h1 t1 h2 t2
-    (EQ: Mcons h1 t1 = Mcons h2 t2):
-  h1 = h2 /\ t1 = t2.
-Proof.
-  unfold Mcons in *. apply Ffix_inj in EQ. inversion EQ. auto.
-Qed.
+  Lemma Mlist_ind l (P: Mlist -> Prop)
+        (BASE: P Mnil)
+        (STEP: forall hd tl 
+                      (IND: forall x, Fn.(mem) tl x -> P x), 
+            P (Mcons hd tl)):
+    P l.
+  Proof.
+    apply ffix_mem_induction. intros. destruct m.
+    - unfold Mnil in BASE. destruct c. apply BASE.
+    - destruct p. unfold Mcons in STEP. apply STEP.
+      intros. apply IND. right. auto.
+  Qed.
 
-Lemma Mcons_inj2 hd tl (EQ: Mcons hd tl = Mnil):
-  False.
-Proof.
-  unfold Mcons, Mnil in *. apply Ffix_inj in EQ. inversion EQ.
-Qed.
+  Definition mfix T (tnil: T) (tcons: M X -> M T -> T) (l: Mlist) : T :=
+    frec_p (fun m => 
+              match m with
+              | inl tt => tnil
+              | inr (mx, mt) => tcons mx mt end) l.
 
-Lemma Mlist_ind l (P: Mlist -> Prop)
-    (BASE: P Mnil)
-    (STEP: forall hd tl 
-             (IND: forall x, mem tl x -> P x), 
-           P (Mcons hd tl)):
-  P l.
-Proof.
-  apply ffix_mem_induction. intros. destruct m.
-  - unfold Mnil in BASE. destruct c. apply BASE.
-  - destruct p. unfold Mcons in STEP. apply STEP.
-    intros. apply IND. right. auto.
-Qed.
+  Lemma mfix_correct_cons T (tnil: T) (tcons: M X -> M T -> T) hd tl : 
+    mfix tnil tcons (Mcons hd tl) = tcons hd (Fn.(map) (mfix tnil tcons) tl).
+  Proof.
+    unfold mfix, Mcons.
+    msimpl. auto.
+  Qed.
 
-Definition mfix T (tnil: T) (tcons: M X -> M T -> T) (l: Mlist) : T :=
-  frec_p (fun m => 
-            match m with
-            | inl tt => tnil
-            | inr (mx, mt) => tcons mx mt end) l.
+  Lemma mfix_correct_nil T (tnil: T) (tcons: M X -> M T -> T) :
+    mfix tnil tcons Mnil = tnil.
+  Proof.
+    unfold mfix, Mnil.
+    msimpl. auto.
+  Qed.
 
-Lemma mfix_correct_cons T (tnil: T) (tcons: M X -> M T -> T) hd tl : 
-  mfix tnil tcons (Mcons hd tl) = tcons hd (map (mfix tnil tcons) tl).
-Proof.
-  unfold mfix, Mcons.
-  msimpl. auto.
-Qed.
+  Definition app' (mys : M Mlist) : Mlist -> M Mlist.
+    apply mfix. apply mys.
+    intros xsh mv.
+    apply ret.
+    apply Mcons. apply xsh.
+    apply mult. apply mv.
+  Defined.
 
-Lemma mfix_correct_nil T (tnil: T) (tcons: M X -> M T -> T) :
-  mfix tnil tcons Mnil = tnil.
-Proof.
-  unfold mfix, Mnil.
-  msimpl. auto.
-Qed.
-
-End Mlist.
-Arguments Mlist M {H} {H0} {H1} X.
-
-
-Module Mlist_Append.
-
-Definition app' M `{SMonad M} {X} (mys : M (Mlist M X)) : Mlist M X -> M (Mlist M X).
-  apply mfix. apply mys.
-  intros xsh mv.
-  apply ret.
-  apply Mcons. apply xsh.
-  apply mult. apply mv.
-Defined.
-
-(*
+    (*
 Definition app' M `{SMonad M} {X} (mys : M (Mlist M X))
  :=
   mfix mys (fun (xsh : M X) (mv : M (Mlist M X)) => ret (Mlist M X) (Mcons X xsh (mult _ mv))).
-*)
+     *)
 
-Definition app M `{SMonad M} {X} (mxs mys : M (Mlist M X)) :=
-  bind (app' mys) mxs.
+  Definition app (mxs mys : M Mlist) :=
+    bind (app' mys) mxs.
 
-Lemma app'_bind M `{SMonad M} {X} (mys : M (Mlist M X)) hd tl :
-  app' mys (Mcons X hd tl) =
-  ret (Mlist M X) (Mcons X hd (bind (app' mys) tl)).
-Proof.
-  unfold app'. apply mfix_correct_cons.
-Qed.
+  Lemma app'_bind (mys : M Mlist) hd tl :
+    app' mys (Mcons hd tl) =
+    ret Mlist (Mcons hd (bind (app' mys) tl)).
+  Proof.
+    unfold app'. apply mfix_correct_cons.
+  Qed.
 
-Theorem app'_assoc : forall M `{SMonad M} {X} (mys mzs : M (Mlist M X)) xs,
-    app (app' mys xs) mzs = app' (app mys mzs) xs.
-Proof.
-  intros. apply (Mlist_ind xs).
-  - unfold app'. repeat rewrite mfix_correct_nil. auto.
-  - intros. unfold app. rewrite app'_bind. rewrite app'_bind.
-    rewrite bind_law_1. rewrite app'_bind.
-    f_equal. f_equal.
-    rewrite bind_law_3.
-    unfold bind. f_equal. 
-    apply map_pointwise. apply IND. 
-Qed.
+  Theorem app'_assoc : forall (mys mzs : M Mlist) xs,
+      app (app' mys xs) mzs = app' (app mys mzs) xs.
+  Proof.
+    intros. apply (Mlist_ind xs).
+    - unfold app'. repeat rewrite mfix_correct_nil. auto.
+    - intros. unfold app. rewrite app'_bind. rewrite app'_bind.
+      rewrite bind_law_1. rewrite app'_bind.
+      f_equal. f_equal.
+      rewrite bind_law_3.
+      unfold bind. f_equal. 
+      apply map_pointwise. apply IND. 
+  Qed.
 
-Theorem app_assoc : forall M `{SMonad M} {X} (mys mzs mxs : M (Mlist M X)),
-    app (app mxs mys) mzs = app mxs (app mys mzs).
-Proof.
-  intros. unfold app.
-  rewrite bind_law_3. f_equal.
-  extensionality x. apply app'_assoc.
-Qed.
+  Theorem app_assoc : forall (mys mzs mxs : M Mlist),
+      app (app mxs mys) mzs = app mxs (app mys mzs).
+  Proof.
+    intros. unfold app.
+    rewrite bind_law_3. f_equal.
+    extensionality x. apply app'_assoc.
+  Qed.
 
-End Mlist_Append.
+End monad.
