src/inductive.v
@@ -8,438 +8,77 @@ Set Automatic Coercions Import.
 
 Require Import Functor SPFunctor spec.
 
-Module RINDUCTIVE : INDUCTIVE.
-
-Section FFix.
-  Variable PF : Type -> Type.
-  Context `{SPF : SPFunctor PF}.
-
-  Inductive ufix: Type :=
-  | Ufix: UF (@Sh1 _ _ _ SPF) (@Sh2 _ _ _ SPF) ufix -> ufix
-  .
-
-  Inductive range: forall (u:ufix), Prop :=
-  | Range
-      (m: PF ufix)
-      (MEM: forall u, mem (emb _ m) u -> range u):
-      range (Ufix (emb _ m))
-  .
-
-  Definition ffix := sig range.
-
-  Definition ffix_to_ufix (x:ffix): ufix := proj1_sig x.
-
-  Lemma Ffix_range (x: PF ffix) : range (Ufix (emb _ (map ffix_to_ufix x))).
-  Proof.
-    constructor. intros.
-    rewrite MAP_COMMUTE in H1. inv H1. simplify.
-    destruct (emb _ x d) eqn : EQ; [| inv MEM]; simplify.
-    subst. destruct i. auto.
-  Defined. 
-
-  Definition Ffix (x: PF ffix) : ffix :=
-    @exist _ _ (Ufix (emb _ (map ffix_to_ufix x))) (Ffix_range x).
-
-  Lemma ffix_des0' u (R:range u): ex (unique (fun m => u = Ufix (emb _ m))).
-  Proof.
-    inv R. exists m. split; auto.
-    intros. inversion H1. apply INJECTIVE. auto.
-  Qed.
-
-  Definition ffix_des0 u (R:range u) : PF ufix :=
-    proj1_sig (constructive_definite_description _ (ffix_des0' R)).
-
-  Lemma ffix_des0_correct m f: ffix_des0 (Range m f) = m.
-  Proof.
-    unfold ffix_des0.
-    destruct (constructive_definite_description
-                 (fun m0 : PF ufix => Ufix (emb _ m) = Ufix (emb _ m0))
-                 (ffix_des0' (Range m f))) eqn : EQ.
-    inversion e. apply INJECTIVE in H2. eauto.
-  Defined.
-
-  Definition ffix_des1 u (R:range u) x (MEM: mem (ffix_des0 R) x): ffix.
-  Proof.
-    exists x.
-    destruct R. apply MEM0. rewrite ffix_des0_correct in MEM.
-    apply MEM_COMMUTE in MEM. auto.
-  Defined.
-
-  Definition ffix_des (f:ffix): PF ffix :=
-    map_dep (ffix_des0 (proj2_sig f)) (ffix_des1 (proj2_sig f)).
-
-  Inductive ufix_ord: forall (x y:ufix), Prop :=
-  | Ufix_ord x u (IN: mem u x): ufix_ord x (Ufix u)
-  .
-
-  Lemma ufix_ord_wf: well_founded ufix_ord.
-  Proof.
-    unfold well_founded. fix 1. intro. destruct a.
-    constructor. intros.
-    inv H1. inversion IN. simplify.
-    destruct (u d); [| inv MEM].
-    specialize (ufix_ord_wf i).
-    rewrite MEM in ufix_ord_wf.
-    apply ufix_ord_wf.
-  Qed.
-
-  Inductive ffix_ord': forall (x y:ffix), Prop :=
-  | Ffix_ord x y PX PY (ORD: ufix_ord x y): ffix_ord' (@exist _ _ x PX) (@exist _ _ y PY)
-  .
-
-  Definition ffix_ord := ffix_ord'.
-
-  Lemma ffix_ord_ufix_ord x y (ORD: ffix_ord x y):
-    ufix_ord (ffix_to_ufix x) (ffix_to_ufix y).
-  Proof.
-    inv ORD. auto.
-  Qed.
-
-  Lemma acc_preserve X Y (f: X -> Y) (Rx : X -> X -> Prop) (Ry : Y -> Y -> Prop)
-        (SUB: forall x1 x2 (RE: Rx x1 x2), Ry (f x1) (f x2))
-        (WF: well_founded Ry) y
-    : forall x, y = f x /\ Acc Ry y -> Acc Rx x.
-  Proof.
-    apply (@Fix Y Ry WF (fun a =>  forall x : X, a = f x /\ Acc Ry a -> Acc Rx x)).
-    intros. destruct H2. subst.
-    constructor. intros. eauto.
-  Qed.
-
-  Lemma sub_wellorder X Y (f: X -> Y) (Rx : X -> X -> Prop) (Ry : Y -> Y -> Prop)
-        (SUB: forall x1 x2 (RE: Rx x1 x2), Ry (f x1) (f x2)) (WF: well_founded Ry) 
-    : well_founded Rx.
-  Proof.
-    unfold well_founded. intros. apply (@acc_preserve _ _ f Rx _ SUB WF (f a)). auto.
-  Qed.
-
-  Lemma ffix_ord_wf: well_founded ffix_ord.
-  Proof.
-    apply (sub_wellorder _ _ ffix_ord_ufix_ord ufix_ord_wf).
-  Qed.
-
-  Lemma ffix_ord_induction x
-        (P: ffix -> Prop)
-        (STEP: forall y, (forall x, ffix_ord x y -> P x) -> P y) :
-    P x.
-  Proof.
-    apply (Fix ffix_ord_wf). apply STEP.
-  Qed.
-
-  Lemma range_unique2 : forall (x1 x2: ufix) p1 p2,
-    x1 = x2 -> exist range x1 p1 = exist range x2 p2.
-  Proof.
-    intros. subst.
-    replace p1 with p2. auto.
-    apply proof_irrelevance.
-  Qed.
-
-  Lemma Ufix_inj u1 u2 (EQ: Ufix u1 = Ufix u2) : u1 = u2.
-  Proof.
-    inversion EQ. auto.
-  Qed.
-
-  Lemma Ffix_inj x1 x2 (EQ: Ffix x1 = Ffix x2) : x1 = x2.
-  Proof.
-    unfold Ffix in EQ.
-    apply eq_sig_fst in EQ. apply Ufix_inj in EQ.
-    apply INJECTIVE.
-    extensionality s. apply equal_f with s in EQ.
-    repeat rewrite MAP_COMMUTE in EQ.
-    simplify.
-    destruct (emb _ x1 s);
-    destruct (emb _ x2 s); inversion EQ; auto.
-    destruct i, i0. simplify. subst.
-    f_equal. f_equal. apply proof_irrelevance.
-  Qed.
-
-  Lemma des_correct1 x: Ffix (ffix_des x) = x.
-  Proof.
-    destruct x. destruct r. unfold Ffix.
-    apply range_unique2.
-    f_equal. f_equal. unfold ffix_des.
-    rewrite MAP_DEP; auto.
-    unfold ffix_des0.
-    destruct (constructive_definite_description
-                (fun m0 : PF ufix =>
-                   ` (exist range (Ufix (emb _ m)) (Range m MEM)) = Ufix (emb _ m0))
-                (ffix_des0' (proj2_sig (exist range (Ufix (emb _ m)) (Range m MEM)))))
-             eqn : EQ.
-    unfold proj1_sig in *. inversion e.
-    apply INJECTIVE in H2. auto.
-  Qed.
-
-  Lemma des_correct2 x: ffix_des (Ffix x) = x.
-  Proof.
-    apply Ffix_inj.
-    apply des_correct1.
-  Qed.
-
-  Definition ffix_ord_c := clos_trans_n1 ffix_ord.
-
-  Lemma ffix_ord_c_wf : well_founded ffix_ord_c.
-  Proof.
-    unfold well_founded. intro. apply (ffix_ord_induction a).
-    intros.
-    constructor. intros.
-    destruct H2.
-    - apply H1, H2.
-    - specialize (H1 y H2).
-      destruct H1. eauto.
-  Qed.
-
-  Lemma ord_transtive x y z (Rxy: ffix_ord_c x y) (Ryz: ffix_ord_c y z) :
-    ffix_ord_c x z.
-  Proof.
-  revert Ryz. revert Rxy.
-  apply (ffix_ord_induction z).
-  intros.
-  destruct Ryz.
-  - apply (tn1_trans _ _ _ _ _ H2 Rxy).
-  - specialize (H1 _ H2 Rxy Ryz).
-    apply (tn1_trans _ _ _ _ _ H2 H1).
-  Qed.
-
-  Definition v_get y (x: @less_ones _ ffix_ord_c y) : ffix :=
-    match x with
-    | @w_ord _ _ _ x' _ => x' end.
-
-  Lemma ffix_str_induction x
-        (P: ffix -> Prop)
-        (STEP: forall y, (forall x, ffix_ord_c x y -> P x) -> P y) :
-    P x.
-  Proof.
-    apply (Fix ffix_ord_c_wf). apply STEP.
-  Qed.
-
-  Definition frec_d (P: ffix -> Type)
-      (FIX: forall m (FN: forall y, ffix_ord_c y m -> P y), P m) : forall x, P x :=
-    Fix ffix_ord_c_wf _ FIX.
-
-  Definition frec T
-      (FIX: forall m (FN: forall y, ffix_ord_c y m -> T), T) x : T :=
-    Fix ffix_ord_c_wf _ FIX x.
-
-  Lemma Fix_F_eq A (R : A -> A -> Prop) (P : A -> Type) (F : forall x: A, (forall y:A, R y x -> P y) -> P x) :
-    forall (x : A) (r: Acc R x),
-    @F x (fun (y : A) (p : R y x) => @Fix_F A R P F y (@Acc_inv A R x r y p)) = Fix_F P F r.
-  Proof.
-    intros. destruct r. simpl. auto.
-  Qed.
-
-  Lemma Fix_correct A (R : A -> A -> Prop) (P : A -> Type) (F : forall x: A, (forall y:A, R y x -> P y) -> P x) (W : well_founded R) :
-    forall x, F x (fun y _ => (Fix W P F y)) = Fix W P F x.
-  Proof.
-    intros. unfold Fix.
-    rewrite <- (Fix_F_eq _ _ (W x)).
-    f_equal. extensionality s1. extensionality s2.
-    f_equal. apply proof_irrelevance.
-  Qed.
-
-  Lemma frec_red T
-        (FIX: forall m (FN: forall y, ffix_ord_c y m -> T), T) x :
-    frec FIX (Ffix x) = FIX (Ffix x) (fun y _ => frec FIX y).
-  Proof.
-    unfold frec. 
-    rewrite <- Fix_correct. auto.
-  Qed.
-
-  Lemma frec_d_red (P: ffix -> Type)
-      (FIX: forall m (FN: forall y, ffix_ord_c y m -> P y), P m) x :
-    frec_d P FIX (Ffix x) 
-    = FIX (Ffix x) (fun y _ => frec_d P FIX y).
-  Proof.
-    unfold frec_d. 
-    rewrite <- Fix_correct. auto.
-  Qed.
-
-  Definition ord_correct m x : mem m x <-> ffix_ord x (Ffix m).
-  Proof.
-    split; intros.
-    - destruct x.
-      constructor. constructor. rewrite MAP_COMMUTE. simplify.
-      apply MEM_COMMUTE in H1.
-      inv H1. simplify. destruct (emb _ m d) eqn : EQ; [| inv MEM].
-      apply (Function_mem _ _ d). simplify.
-      rewrite EQ. rewrite MEM. simplify. auto.
-    - inv H1. inv ORD. inv IN. rewrite MAP_COMMUTE in MEM. simplify.
-      apply MEM_COMMUTE.
-      apply (Function_mem _ _ d). simplify.
-      destruct (emb _ m d); inversion MEM.
-      subst. destruct i. simplify. f_equal.
-      apply proof_irrelevance.
-  Qed.
-
-  Lemma ffix_mem_induction x (P: ffix -> Prop)
-        (STEP: forall m (IND: forall y, mem m y -> P y), P (Ffix m)):
-    P x.
-  Proof.
-    assert (H1 : forall m (IND: forall y, ffix_ord y m -> P y), P m). intros.
-    rewrite <- (des_correct1 m) in *. apply STEP.
-    intros. apply IND.
-    apply ord_correct, H1.
-    apply (ffix_ord_induction x _ H1).
-  Qed.
-
-  Definition ffix_des_ord' u (R: range u): forall x (MEM: mem (ffix_des0 R) x),
-      @less_ones _ ffix_ord_c (exist _ _ R).
-  Proof.
-    intros.
-    apply (@w_ord _ _ _ (ffix_des1 R x MEM)).
-    destruct R. apply tn1_step. constructor. constructor.
-    rewrite <- MEM_COMMUTE.
-    rewrite ffix_des0_correct in MEM. auto.
-  Defined.
-
-  Definition ffix_des_ord (x: ffix) : PF (less_ones x) :=
-    match x with
-    | exist _ _ p => map_dep _ (ffix_des_ord' p) end.
-
-  Definition order_part m : forall x, mem m x -> ffix_ord_c x (Ffix m).
-    intros. destruct x. unfold Ffix.
-    repeat constructor.
-    rewrite MEM_COMMUTE in H1. rewrite MAP_COMMUTE.
-    inv H1. simplify.
-    apply (Function_mem _ _ d). simplify.
-    destruct (emb _ m d); inversion MEM. simplify. auto.
-  Qed.
-
-  Lemma des_ord_correct m 
-    : ffix_des_ord (Ffix m) 
-      = map_dep m (fun x r => w_ord _ (order_part m x r)).
-  Proof.
-    apply (map_injective (fun x => proj1_sig (v_get x))).
-    - intros. destruct x1, x2. destruct x, x0.
-      simpl in EQ. subst.
-      assert (EQ := proof_irrelevance _ r r0). subst.
-      f_equal. apply proof_irrelevance.
-    - simplify. rewrite MAP_DEP; [| intros; auto].
-      unfold Ffix_range. rewrite (ffix_des0_correct (map (ffix_to_ufix) m) _).
-      replace (map (fun x : _ => ` (v_get x))
-                   (map_dep m
-                            (fun (x : ffix) (r : mem m x) =>
-                               w_ord x (order_part m x r)))) with
-          (map (@proj1_sig _ _) (map (@v_get _) (map_dep m
-                                                         (fun (x : ffix) (r : mem m x) =>
-                                                            w_ord x (order_part m x r))))); [| apply MAP_COMPOSE].
-      f_equal. rewrite MAP_DEP; auto.
-  Qed.
-
-  Definition frec_p T (f: PF T -> T) : ffix -> T :=
-    frec (fun (m: ffix) g =>
-            let g' (m': @less_ones _ ffix_ord_c m) : T :=
-                match m' with
-                | @w_ord _ _ _ m'' r => g m'' r end in
-            f (map g' (ffix_des_ord m))).
-
-  Lemma frec_p_red T (f: PF T -> T) m :
-    frec_p f (Ffix m) = f (map (frec_p f) m).
-  Proof.
-    unfold frec_p. rewrite frec_red.
-    f_equal. rewrite des_ord_correct.
-    remember (frec
-           (fun (m0 : ffix) (g : forall y : ffix, ffix_ord_c y m0 -> T) =>
-            f
-              (map
-                 (fun m'0 : @less_ones _ ffix_ord_c m0 =>
-                  match m'0 with
-                  | w_ord m''0 r0 => g m''0 r0
-                  end) (ffix_des_ord m0)))) as g.
-    replace (fun m' : @less_ones _ ffix_ord_c (Ffix m) =>
-     match m' with
-     | w_ord m'' _ => g m''
-     end) with (fun m' => g (@v_get (Ffix m) m'));
-      [| extensionality s; destruct s; auto].
-    replace (map (fun m' : less_ones (Ffix m) => g (v_get m'))
-    (map_dep m
-       (fun (x : ffix) (r : mem m x) =>
-        w_ord x (order_part m x r)))) with
-        (map g (map (@v_get _ ) (map_dep m
-       (fun (x : ffix) (r : mem m x) =>
-        w_ord x (order_part m x r))))); [| apply Functor.MAP_COMPOSE].
-    f_equal. apply MAP_DEP. auto.
-  Qed.
-
-
-End FFix.
-
-End RINDUCTIVE.
-
 Section inductive.
 
   Variable PF : Type -> Type.
-  Context `{H : FunctorData PF}.
-  Context `{H0 : @SFunctorData PF _}.
-  Context `{SPF : @SPFunctor PF _ _}.
+  Context `{SPF : SPFunctor PF}.
 
-  Definition ffix : Type := @RINDUCTIVE.ffix PF _ _ _. (* inductive type *)
+  Definition ffix : Type. Admitted. (* inductive type *)
 
-  Definition Ffix : PF ffix -> ffix := @RINDUCTIVE.Ffix PF _ _ _. (* constructor *)
+  Definition Ffix : PF ffix -> ffix. Admitted. (* constructor *)
 
-  Definition ffix_des : ffix -> PF ffix := @RINDUCTIVE.ffix_des PF _ _ _. (* destructor *)
+  Definition ffix_des : ffix -> PF ffix. Admitted. (* destructor *)
 
-  Definition Ffix_inj : forall x1 x2 (EQ: Ffix x1 = Ffix x2), x1 = x2 := @RINDUCTIVE.Ffix_inj PF _ _ _.
+  Definition Ffix_inj : forall x1 x2 (EQ: Ffix x1 = Ffix x2), x1 = x2. Admitted.
   (* constructors are injective *)
 
-  Definition des_correct1 : forall x, Ffix (ffix_des x) = x := @RINDUCTIVE.des_correct1 PF _ _ _.
+  Definition des_correct1 : forall x, Ffix (ffix_des x) = x. Admitted.
 
-  Definition des_correct2 : forall x, ffix_des (Ffix x) = x := @RINDUCTIVE.des_correct2 PF _ _ _.
+  Definition des_correct2 : forall x, ffix_des (Ffix x) = x. Admitted.
   (* these say that destructors are the inverse of constructors *)
-
 
 (* order and induction principle *)
 
-  Definition ffix_ord : ffix -> ffix -> Prop := @RINDUCTIVE.ffix_ord PF _ _ _. (* order on ffix *)
+  Definition ffix_ord : ffix -> ffix -> Prop. Admitted. (* order on ffix *)
 
   Definition ffix_ord_c := @clos_trans_n1 ffix ffix_ord. (* closure of ffix_ord *)
 
-  Definition ord_correct : forall m x, mem m x <-> ffix_ord x (Ffix m) := @RINDUCTIVE.ord_correct PF _ _ _.
+  Definition ord_correct : forall m x, SPF.(mem) m x <-> ffix_ord x (Ffix m). Admitted.
   (* membership relations in SPFunctor became order on ffix *)
 
   Definition ord_transitive : forall x y z (Rxy: ffix_ord_c x y) (Ryz: ffix_ord_c y z),
-      ffix_ord_c x z := @RINDUCTIVE.ord_transtive PF _ _ _.
+      ffix_ord_c x z. Admitted.
 
-  Definition ffix_ord_wf: well_founded ffix_ord := @RINDUCTIVE.ffix_ord_wf PF _ _ _.
+  Definition ffix_ord_wf: well_founded ffix_ord. Admitted.
 
-  Definition ffix_ord_c_wf : well_founded ffix_ord_c := @RINDUCTIVE.ffix_ord_c_wf PF _ _ _.
+  Definition ffix_ord_c_wf : well_founded ffix_ord_c. Admitted.
   (* well order *)
 
-  Definition ffix_des_ord : forall (x: ffix), PF (less_ones x) := @RINDUCTIVE.ffix_des_ord PF _ _ _.
+  Definition ffix_des_ord : forall (x: ffix), PF (@less_ones ffix ffix_ord_c x). Admitted.
   (* destruct with order *)
 
-  Definition order_part : forall m x, mem m x -> ffix_ord_c x (Ffix m) := @RINDUCTIVE.order_part PF _ _ _.
+  Definition order_part : forall m x, SPF.(mem) m x -> ffix_ord_c x (Ffix m). Admitted.
   (* users don't need to know this *)
 
   Definition des_ord_correct : forall (m : PF ffix),
-      ffix_des_ord (Ffix m) = map_dep m (fun x r => w_ord _ (order_part m x r)) := @RINDUCTIVE.des_ord_correct PF _ _ _.
-
+      ffix_des_ord (Ffix m) = SPF.(map_dep) m (fun x r => w_ord _ (order_part m x r)). Admitted.
 (* induction principles with different forms *)
 
   Definition ffix_ord_induction : forall x (P: ffix -> Prop)
         (STEP: forall y, (forall x, ffix_ord x y -> P x) -> P y),
-    P x := @RINDUCTIVE.ffix_ord_induction PF _ _ _.
+    P x. Admitted.
 
   Definition ffix_str_induction : forall x (P: ffix -> Prop)
         (STEP: forall y, (forall x, ffix_ord_c x y -> P x) -> P y),
-    P x := @RINDUCTIVE.ffix_str_induction PF _ _ _.
+    P x. Admitted.
     (* strong induction *)
 
   Definition ffix_mem_induction : forall x (P: ffix -> Prop)
-        (STEP: forall m (IND: forall y, mem m y -> P y), P (Ffix m)),
-    P x := @RINDUCTIVE.ffix_mem_induction PF _ _ _.
-
+        (STEP: forall m (IND: forall y, SPF.(mem) m y -> P y), P (Ffix m)),
+    P x. Admitted.
 
 (* recursive function *)
 
   Definition frec : forall T (FIX: forall m (FN: forall y, ffix_ord_c y m -> T), T),
-      ffix -> T := @RINDUCTIVE.frec PF _ _ _.
+      ffix -> T. Admitted. 
 
   Definition frec_d: forall (P: ffix -> Type)
                           (FIX: forall m (FN: forall y, ffix_ord_c y m -> P y), P m),
-      forall x : ffix, P x := @RINDUCTIVE.frec_d PF _ _ _.
+      forall x : ffix, P x. Admitted.
   (* dependent functions *)
 
   Definition frec_p : forall T (f: PF T -> T),
-      ffix -> T := @RINDUCTIVE.frec_p PF _ _ _.
+      ffix -> T. Admitted.
   (* primitive recursion : simple but not general *)
 
 
@@ -447,14 +86,14 @@ Section inductive.
 
   Definition frec_red : forall T
       (FIX: forall m (FN: forall y, ffix_ord_c y m -> T), T) x,
-    frec FIX (Ffix x) = FIX (Ffix x) (fun y _ => frec FIX y) := @RINDUCTIVE.frec_red PF _ _ _.
+    frec FIX (Ffix x) = FIX (Ffix x) (fun y _ => frec FIX y). Admitted.
 
   Definition frec_d_red : forall (P: ffix -> Type)
       (FIX: forall m (FN: forall y, ffix_ord_c y m -> P y), P m) x,
-    frec_d P FIX (Ffix x) = FIX (Ffix x) (fun y _ => frec_d P FIX y) := @RINDUCTIVE.frec_d_red PF _ _ _.
+    frec_d P FIX (Ffix x) = FIX (Ffix x) (fun y _ => frec_d P FIX y). Admitted.
 
   Definition frec_p_red : forall T (f: PF T -> T) m,
-    frec_p f (Ffix m) = f (map (frec_p f) m) := @RINDUCTIVE.frec_p_red PF _ _ _.
+    frec_p f (Ffix m) = f (SPF.(map) (frec_p f) m). Admitted.
 
 End inductive.
 
@@ -478,6 +117,5 @@ Ltac msimpl_in H := repeat (autounfold in H;
                             repeat unfold id in H;
                             simpl in H).
 
-Arguments ffix PF {H} {H0} {SPF}.
-Arguments Ffix PF {H} {H0} {SPF}.
-Arguments ffix_des {PF} {H} {H0} {SPF}.
+Arguments ffix PF {SPF}.
+Arguments Ffix PF {SPF}.
